stack_map update, proof refactor

theories/iris/examples/stack/function/stack_map.v
@@ -21,62 +21,884 @@ Section stack.
  
 Section code.
 
-Definition stack_map :=
-  validate_stack 1 ++
+(*
+  map: [i32, i32] -> []
+  locals declared: [i32, i32]
+
+  Given a stack pointer and a function reference from table 0, apply the function to all elements of the stack and
+  storing the results in the original stack.
+
+  Implementation is done via looping through the stack, loading each element and call_indirect the function, then
+  store the element back to the original address. The loop variable represents the top address that *has* been 
+  dealt with, to avoid u32 overflow. The loop upper bound is then simply the stack top pointer, retrieved from the value
+  stored in the stack pointer address.
+
+  The spec of the map function allows description of a relationship between the old and the new stack via an arbitrary
+  assertion, which is given by the spec of the input function reference.
+  
+  Returns nothing. Can trap if the stack validation traps, or any of the function application traps.
+
+  Parameters/Locals:
+  0 (input)     stack pointer
+  1 (input)     function reference from table 0, which must be of type [i32] -> [i32]
+  2             temporary variable storing the loop variable
+  3             temporary variable storing the loop upper bound
+*)
+  
+Definition map_initialise :=
   [
-    BI_get_local 1 ;
+    BI_get_local 0 ;
     BI_load T_i32 None N.zero N.zero ;
     BI_set_local 3 ;
-    BI_get_local 1 ;
-    i32const 4 ;
-    BI_binop T_i32 (Binop_i BOI_add) ;
-    BI_set_local 2 ;
-    BI_block (Tf [] [])
-             [BI_loop (Tf [] [])
-                      [BI_get_local 2 ;
-                       BI_get_local 3 ;
-                       BI_relop T_i32 (Relop_i (ROI_ge SX_U)) ;
-                       BI_br_if 1 ;
-                       BI_get_local 2 ;
-                       BI_get_local 2 ;
-                       BI_get_local 2 ;
-                       BI_load T_i32 None N.zero N.zero ;
-                       BI_get_local 0 ;
-                       BI_call_indirect 1 ;
-                       BI_store T_i32 None N.zero N.zero ;
-                       i32const 4 ;
-                       BI_binop T_i32 (Binop_i BOI_add) ;
-                       BI_set_local 2 ;
-                       BI_br 0]
-             ]
+  
+    BI_get_local 0 ;
+    BI_set_local 2
   ].
 
+Definition map_loop_body :=
+  [
+    (* Check if the loop is done *)
+    BI_get_local 2 ;
+    BI_get_local 3 ;
+    BI_relop T_i32 (Relop_i ROI_eq) ;
+    BI_br_if 1 ;
 
+    (* Update the loop variable and add a copy to the stack (for storing later) *)
+    BI_get_local 2 ;
+    i32const 4 ;
+    BI_binop T_i32 (Binop_i BOI_add) ;
+    BI_tee_local 2 ;
+
+    (* Load the stack element, apply the function and store the result back to the stack *)
+    BI_get_local 2 ;
+    BI_load T_i32 None N.zero N.zero ;
+    BI_get_local 1 ;
+    BI_call_indirect 1 ;
+    BI_store T_i32 None N.zero N.zero ;
+
+    (* Keep the loop alive *)
+    BI_br 0
+  ].
+
+Definition map_op :=
+  map_initialise ++
+  [
+    BI_block (Tf [] [])
+             [BI_loop (Tf [] []) map_loop_body]
+  ].
+
+Definition stack_map :=
+  validate_stack 0 ++ validate_stack_bound 0 ++ map_op.
 
 End code.
+
+Lemma stack_pure v s n:
+  isStack v s n -∗
+  ⌜(two16 | v)%Z⌝ ∗ ⌜(0 <= v <= ffff0000)%Z⌝ ∗ ⌜(length s < two14)%Z⌝ ∗ isStack v s n.
+Proof.
+  iIntros "Hs".
+  repeat iSplit => //; by iDestruct "Hs" as "(% & (% & %) & % & ?)".
+Qed.
+
+
+Lemma stack_load_0 v s n f E:
+  ⌜ f.(f_inst).(inst_memory) !! 0 = Some n ⌝ -∗
+  isStack v s n -∗
+  ↪[frame] f -∗
+  WP [AI_basic (BI_const (value_of_int v)); AI_basic (BI_load T_i32 None N.zero N.zero)] @ E
+  {{ w, ⌜ w = immV [value_of_int (v + length s * 4)] ⌝ ∗ isStack v s n ∗ ↪[frame] f }}.
+Proof.
+  iIntros "%Hinstmem Hs Hf" => /=.
+  
+  iDestruct (stack_pure with "Hs") as "(%Hdiv & %Hvb & %Hlens & Hs)".
+  
+  iApply (wp_wand with "[Hs Hf]").
+  iApply wp_load => //; last first.
+  { unfold isStack.
+    iDestruct "Hs" as "(% & % & % & Hn & Hrest)".
+    iDestruct (i32_wms with "Hn") as "Hn".
+    rewrite N.add_0_r.
+    simpl.
+    rewrite Wasm_int.Int32.Z_mod_modulus_eq.
+    rewrite Z.mod_small; last by unfold ffff0000 in Hvb; rewrite u32_modulus; lia.
+    unfold bits.
+    instantiate (1 := VAL_int32 _) => /=.
+    iFrame.
+    iNext.
+    instantiate (1 := λ w, (⌜ w = immV _ ⌝ ∗ _)%I) => /=.
+    iSplit => //.
+    by iApply "Hrest".
+  }
+  { done. }
+  { iIntros (w) "(((-> & Hrest) & Hn) & Hf)".
+    iSplit => //.
+    iFrame.
+    repeat iSplit => //=.
+    rewrite Wasm_int.Int32.Z_mod_modulus_eq.
+    rewrite Z.mod_small; last by unfold ffff0000 in Hvb; rewrite u32_modulus; lia.
+    rewrite N.add_0_r.
+    by iApply i32_wms.
+  }
+Qed.
+
+Lemma stack_load_j v s n f E j sv:
+  ⌜ f.(f_inst).(inst_memory) !! 0 = Some n ⌝ -∗
+  ⌜ s !! (Z.to_nat j) = Some sv ⌝ -∗
+  ⌜ (0 <= j < length s)%Z ⌝ -∗
+  isStack v s n -∗
+  ↪[frame] f -∗
+  WP [AI_basic (BI_const (value_of_int (v + length s * 4 - 4 * j))); AI_basic (BI_load T_i32 None N.zero N.zero)] @ E
+  {{ w, ⌜ w = immV [VAL_int32 sv] ⌝ ∗ isStack v s n ∗ ↪[frame] f }}.
+Proof.
+  iIntros "%Hinstmem %Hsv %Hjbound Hs Hf" => /=.
+
+  iDestruct (stack_pure with "Hs") as "(%Hdiv & %Hvb & %Hlens & Hs)".
+  
+  assert (0 <= j < 16383)%Z as Hjb; first by unfold two14 in Hlens; lia.
+  
+  iApply (wp_wand with "[Hs Hf]").
+  iApply wp_load => //; last first.
+  { unfold isStack.
+    iDestruct "Hs" as "(_ & _ & _ & Hn & Hcontent & Hrest)".
+    iDestruct (big_sepL_lookup_acc with "Hcontent") as "(Hj & Hcrest)" => //=.
+    rewrite Wasm_int.Int32.Z_mod_modulus_eq.
+    rewrite Z.mod_small; last first.
+    { unfold ffff0000 in Hvb; unfold two14 in Hlens; rewrite u32_modulus.
+      remember (length s) as x.
+      rewrite - Heqx.
+      lia.
+    }
+    rewrite N.add_0_r.
+    iDestruct (i32_wms with "Hj") as "Hj".
+    unfold bits.
+    instantiate (1 := VAL_int32 sv) => /=.
+    iSplitR "Hf Hj"; last first.
+    iFrame "Hf".
+    replace (4*Z.to_nat j)%Z with (4*j)%Z => //.
+    lia.
+    instantiate (1 := λ w, (⌜ w = immV [VAL_int32 sv] ⌝ ∗ _)%I).
+    iIntros "!>" => /=.
+    iSplit => //.
+    iCombine "Hn Hrest Hcrest" as "H".
+    by iApply "H".
+  }
+  { done. }
+
+  iIntros (w) "(((-> & Hn & Hrest & Hcrest) & Hj) & Hf)".
+  iSplit => //.
+  iFrame.
+  repeat iSplit => //=.
+  iApply "Hcrest".
+  iDestruct (i32_wms with "Hj") as "Hj".
+  rewrite Wasm_int.Int32.Z_mod_modulus_eq.
+  rewrite Z.mod_small; last first.
+  { unfold ffff0000 in Hvb; unfold two14 in Hlens; rewrite u32_modulus.
+    remember (length s) as x.
+    rewrite - Heqx.
+    lia.
+  }
+  rewrite N.add_0_r.
+  replace (4*Z.to_nat j)%Z with (4*j)%Z => //.
+  lia.  
+Qed.
+
+Lemma stack_store_j v (s: list i32) n f E j sv (v0: i32):
+  ⌜ f.(f_inst).(inst_memory) !! 0 = Some n ⌝ -∗
+  ⌜ s !! (Z.to_nat j) = Some sv ⌝ -∗
+  ⌜ (0 <= j < length s)%Z ⌝ -∗
+  isStack v s n -∗
+  ↪[frame] f -∗
+  WP [AI_basic (BI_const (value_of_int (v + length s * 4 - 4 * j))); AI_basic (BI_const (VAL_int32 v0)); AI_basic (BI_store T_i32 None N.zero N.zero)] @ E
+  {{ w, ⌜ w = immV [] ⌝ ∗ isStack v (<[ Z.to_nat j := v0 ]> s) n ∗ ↪[frame] f }}.
+Proof.
+  iIntros "%Hinstmem %Hsv %Hjbound Hs Hf" => /=.
+
+  iDestruct (stack_pure with "Hs") as "(%Hdiv & %Hvb & %Hlens & Hs)".
+  
+  assert (0 <= j < 16383)%Z as Hjb; first by unfold two14 in Hlens; lia.
+  
+  iApply (wp_wand with "[Hs Hf]").
+  iApply wp_store => //; last first.
+  { unfold isStack.
+    iDestruct "Hs" as "(_ & _ & _ & Hn & Hcontent & Hrest)".
+    iDestruct (big_sepL_insert_acc with "Hcontent") as "(Hj & Hcrest)" => //=.
+    rewrite Wasm_int.Int32.Z_mod_modulus_eq.
+    rewrite Z.mod_small; last first.
+    { unfold ffff0000 in Hvb; unfold two14 in Hlens; rewrite u32_modulus.
+      remember (length s) as x.
+      rewrite - Heqx.
+      lia.
+    }
+    rewrite N.add_0_r.
+    iDestruct (i32_wms with "Hj") as "Hj".
+    iSplitR "Hf Hj"; last first.
+    iFrame "Hf".
+    replace (4*Z.to_nat j)%Z with (4*j)%Z => //.
+    lia.
+    instantiate (1 := λ w, (⌜ w = immV [] ⌝ ∗ _)%I).
+    iIntros "!>" => /=.
+    iSplit => //.
+    iCombine "Hn Hrest Hcrest" as "H".
+    by iApply "H".
+  }
+  { done. }
+
+  iIntros (w) "(((-> & Hn & Hrest & Hcrest) & Hj) & Hf)".
+  iSplit => //.
+  iFrame "Hf".
+  repeat iSplit => //=.
+  { by rewrite insert_length. }
+  repeat rewrite insert_length.
+  iFrame.
+  iApply "Hcrest".
+  iDestruct (i32_wms with "Hj") as "Hj".
+  rewrite Wasm_int.Int32.Z_mod_modulus_eq.
+  rewrite Z.mod_small; last first.
+  { unfold ffff0000 in Hvb; unfold two14 in Hlens; rewrite u32_modulus.
+    remember (length s) as x.
+    rewrite - Heqx.
+    lia.
+  }
+  rewrite N.add_0_r.
+  replace (4*Z.to_nat j)%Z with (4*j)%Z => //.
+  lia.  
+Qed.
 
 
 
 Section specs.
 
+Lemma spec_map_initialise (f: frame) s v n E:
+  ⊢ {{{ ⌜ f.(f_inst).(inst_memory) !! 0 = Some n ⌝ ∗
+        ⌜ f.(f_locs) !! 0 = Some (value_of_int v) ⌝ ∗
+        ⌜ length f.(f_locs) >= 4 ⌝ ∗
+        isStack v s n ∗
+        ↪[frame] f }}}
+    to_e_list map_initialise @ E
+    {{{ w, ⌜ w = immV [] ⌝ ∗
+           isStack v s n ∗
+           ↪[frame] {|
+             f_locs := <[ 2 := value_of_int v ]>
+                       (<[ 3 := value_of_int (v + length s * 4) ]> f.(f_locs));
+             f_inst := f_inst f
+           |}
+    }}}.
+Proof.
+  iIntros "!>" (Φ) "(%Hinstmem & %Hlocs0 & %Hlocs & Hs & Hf) HΦ" => /=.
+
+  iDestruct (stack_pure with "Hs") as "(%Hdiv & %Hvb & %Hlens & Hs)".
+  
+  rewrite separate1.
+  iApply wp_seq.
+  iSplitR; last iSplitL "Hf".
+  2: { iApply wp_get_local => //.
+       by instantiate (1 := λ w, ⌜ w = immV _ ⌝%I).
+  }
+  { by iIntros "(%Habs & _)". }
+  
+  iIntros (w) "(-> & Hf)" => /=.
+  rewrite separate2.
+  iApply wp_seq.
+  instantiate (1 := λ w, (⌜w = immV [_]⌝ ∗ isStack v s n ∗ ↪[frame] f)%I).
+  iSplitR; last iSplitL "Hs Hf".
+  2: { by iApply (stack_load_0 with "[] [$Hs] [$Hf]") => //. }
+  { by iIntros "(%Habs & _)". }
+
+  iIntros (w) "(-> & Hs & Hf)" => /=.
+  rewrite separate2.
+  iApply wp_seq.
+  iSplitR; last iSplitL "Hf".
+  2: { iApply wp_set_local => //.
+       by instantiate (1 := λ w, ⌜ w = immV _ ⌝%I).
+  }
+  { by iIntros "(%Habs & _)". }
+
+  iIntros (w) "(-> & Hf)" => /=.
+  rewrite separate1.
+  iApply wp_seq.
+  iSplitR; last iSplitL "Hf".
+  2: { iApply wp_get_local; last by iApply "Hf".
+       { simpl.
+         rewrite - fmap_insert_set_nth; last lia.
+         by rewrite list_lookup_insert_ne => //.
+       }
+       by instantiate (1 := λ w, ⌜ w = immV _ ⌝%I).
+  }
+  { by iIntros "(%Habs & _)". }
+
+  iIntros (w) "(-> & Hf)" => /=.
+  iApply (wp_wand with "[Hf]").
+  { iApply wp_set_local; last by iApply "Hf".
+    { simpl.
+      rewrite - fmap_insert_set_nth; last lia.
+      rewrite insert_length.
+      lia.
+    }
+    by instantiate (1 := λ w, ⌜ w = immV _ ⌝%I).
+  }
+
+  iIntros (w) "(-> & f)" => /=.
+  iApply "HΦ".
+  iFrame.
+  iSplit => //.
+  
+  erewrite fmap_insert_set_nth => /=; last by rewrite insert_length; lia.
+  erewrite fmap_insert_set_nth => /=; last lia.
+  done.
+Qed.
+
+Lemma spec_map_loop_body_terminate f s v n E j k:
+  ⊢ {{{ ⌜ f.(f_inst).(inst_memory) !! 0 = Some n ⌝ ∗
+        ⌜ f.(f_locs) !! 0 = Some (value_of_int v) ⌝ ∗
+        ⌜ f.(f_locs) !! 2 = Some (value_of_int j) ⌝ ∗
+        ⌜ f.(f_locs) !! 3 = Some (value_of_int k) ⌝ ∗
+        ⌜ j = k ⌝ ∗
+        ⌜ length f.(f_locs) >= 4 ⌝ ∗
+        isStack v s n ∗
+        ↪[frame] f }}}
+    to_e_list map_loop_body @ E
+    {{{ w, ⌜ exists es, w = brV (VH_base 1 [] es) ⌝ ∗
+           isStack v s n ∗ ↪[frame] f
+    }}}.
+Proof.
+  iIntros "!>" (Φ) "(%Hinstmem & %Hlocs0 & %Hlocs2 & %Hlocs3 & <- & %Hlocs & Hs & Hf) HΦ" => /=.
+
+  iDestruct (stack_pure with "Hs") as "(%Hdiv & %Hvb & %Hlens & Hs)".
+
+  rewrite separate1.
+  iApply wp_seq.
+  iSplitR; last iSplitL "Hf".
+  2: { iApply wp_get_local => //.
+       by instantiate (1 := λ w, ⌜ w = immV _ ⌝%I).
+  }
+  { by iIntros "(%Habs & _)". }
+
+  iIntros (w) "(-> & Hf)" => /=.
+  rewrite separate2.
+  iApply wp_seq.
+  instantiate (1 := λ w, (⌜ w = immV [value_of_int j; value_of_int j] ⌝ ∗ ↪[frame] f)%I).
+  iSplitR; last iSplitL "Hf".
+  { by iIntros "(%Habs & _)". }
+  { rewrite separate1.
+    iApply wp_val_app => //.
+    iSplit; first by iIntros "!> (%Habs & _)".
+    by iApply wp_get_local => //.
+  }
+
+  iIntros (w) "(-> & Hf)" => /=.
+  rewrite separate3.
+  iApply wp_seq.
+  iSplitR; last iSplitL "Hf".
+  2: { iApply (wp_relop with "Hf") => //=.
+       rewrite Wasm_int.Int32.eq_true => /=.
+       by instantiate (1 := λ w, ⌜ w = immV _ ⌝%I).
+  }
+  { by iIntros "(%Habs & _)". }
+
+  iIntros (w) "(-> & Hf)" => /=.
+  rewrite separate2.
+  iApply wp_seq.
+  iSplitR; last iSplitL "Hf".
+  2: { iApply (wp_br_if_true with "Hf") => //=.
+       iIntros "!> Hf".
+       instantiate (1 := λ w, (⌜ w = brV (VH_base 1 [] []) ⌝ ∗ ↪[frame] f)%I).
+       iApply wp_value; last by iFrame.
+       done.
+  }
+  { by iIntros "(%Habs & _)". }
+
+  iIntros (w) "(-> & Hf)" => /=.
+  iApply (wp_wand with "[Hf]").
+  { iApply wp_value; last iFrame.
+    { instantiate (1 := brV (VH_base 1 [] _)).
+      rewrite separate1.
+      unfold IntoVal.
+      simpl.
+      done.
+    }
+    { by instantiate (1 := λ w, (⌜ w = brV _ ⌝ ∗ ↪[frame] f)%I); iFrame. }
+  }
+  
+  iIntros (w) "(-> & Hf)" => /=.
+  iApply "HΦ".
+  iFrame.
+  iPureIntro; by eexists.
+Qed.
+
+Lemma spec_map_loop_body_continue f (s: list i32) v n E j fn (sv: i32) j0 a cl
+      (Φ : i32 -> iPropI Σ) (Ψ: i32 -> i32 -> iPropI Σ):
+  ⊢ {{{ ⌜ f.(f_inst).(inst_memory) !! 0 = Some n ⌝ ∗
+        ⌜ f.(f_locs) !! 0 = Some (value_of_int v) ⌝ ∗
+        ⌜ f.(f_locs) !! 1 = Some (VAL_int32 fn) ⌝  ∗
+        ⌜ f.(f_locs) !! 2 = Some (value_of_int (v + (length s) * 4 - 4 * j - 4)) ⌝ ∗
+        ⌜ f.(f_locs) !! 3 = Some (value_of_int (v + (length s) * 4)) ⌝ ∗
+        ⌜ length f.(f_locs) >= 4 ⌝ ∗
+        ⌜ (0 <= j < length s)%Z ⌝ ∗
+        ⌜ s !! (Z.to_nat j) = Some sv ⌝ ∗
+        isStack v s n ∗
+        Φ sv ∗
+            ⌜ f.(f_inst).(inst_types) !! 1 = Some (Tf [T_i32] [T_i32]) ⌝ ∗
+
+            ⌜ f.(f_inst).(inst_tab) !! 0 = Some j0 ⌝ ∗
+            (N.of_nat j0) ↦[wt][ N.of_nat (Wasm_int.nat_of_uint i32m fn) ] (Some a) ∗
+            (N.of_nat a) ↦[wf] cl ∗
+            ⌜ cl_type cl = Tf [T_i32] [T_i32] ⌝ ∗ 
+            (∀ (u : i32) (fc : frame),
+                {{{ Φ u ∗
+                      ⌜ f_inst f = f_inst fc ⌝ ∗
+                       ↪[frame] fc ∗
+                       (N.of_nat j0) ↦[wt][ N.of_nat (Wasm_int.nat_of_uint i32m fn) ] (Some a) ∗
+                       (N.of_nat a) ↦[wf] cl
+                  }}}
+                  [ AI_basic (BI_const (VAL_int32 u)) ;
+                    AI_invoke a ] @ E
+                  {{{ w, (∃ v, ⌜ w = immV [VAL_int32 v] ⌝ ∗ Ψ u v)
+                           ∗ ↪[frame] fc
+                           ∗ (N.of_nat j0) ↦[wt][ N.of_nat (Wasm_int.nat_of_uint i32m fn) ] (Some a) 
+                           ∗ (N.of_nat a) ↦[wf] cl }}}) ∗   
+        ↪[frame] f }}}
+    to_e_list map_loop_body @ E
+    {{{ w, ⌜ w = brV (VH_base 0 [] []) ⌝ ∗
+           (∃ (sv': i32), isStack v (<[Z.to_nat j := sv']> s) n ∗ Ψ sv sv') ∗
+            (N.of_nat j0) ↦[wt][ N.of_nat (Wasm_int.nat_of_uint i32m fn) ] (Some a) ∗
+            (N.of_nat a) ↦[wf] cl ∗
+            ↪[frame]
+            {| f_locs := <[ 2 := value_of_int (v + (length s) * 4 - 4 * j) ]> f.(f_locs);
+               f_inst := f.(f_inst)
+            |}
+    }}}.
+Proof.
+  iIntros "!>" (Ξ) "(%Hinstmem & %Hlocs0 & %Hlocs1 & %Hlocs2 & %Hlocs3 & %Hlocs & %Hjbound & %Hslookup & Hs & HΦ & %Htypes & %Htab & Htab & Hcl & %Hclt & #Hspec & Hf) HΞ" => /=.
+
+  iDestruct (stack_pure with "Hs") as "(%Hdiv & %Hvb & %Hlens & Hs)".
+
+  assert (0 <= j < 16383)%Z as Hjb.
+  { unfold two14 in Hlens. by lias. }
+  
+  rewrite (separate1 (AI_basic _)).
+  iApply wp_seq.
+  iSplitR; last iSplitL "Hf".
+  2: { iApply wp_get_local => //.
+       by instantiate (1 := λ w, ⌜ w = immV _ ⌝%I).
+  }
+  { by iIntros "(%Habs & _)". }
+
+  iIntros (w) "(-> & Hf)" => /=.
+  rewrite separate2.
+  iApply wp_seq.
+  instantiate (1 := λ w, (⌜ w = immV [value_of_int (v + length s * 4 - 4 * j - 4); value_of_int (v + length s * 4)] ⌝ ∗ ↪[frame] f)%I).
+  iSplitR; last iSplitL "Hf".
+  { by iIntros "(%Habs & _)". }
+  { rewrite (separate1 (AI_basic _)).
+    iApply wp_val_app => //.
+    iSplit; first by iIntros "!> (%Habs & _)".
+    by iApply wp_get_local => //.
+  }
+
+  iIntros (w) "(-> & Hf)" => /=.
+  rewrite separate3.
+  iApply wp_seq.
+  iSplitR; last iSplitL "Hf".
+  2: { iApply (wp_relop with "Hf") => //=.
+       rewrite Wasm_int.Int32.eq_false => /=; first by instantiate (1 := λ w, ⌜ w = immV _ ⌝%I).
+       remember (length s) as x.
+       rewrite - Heqx.
+       move => Hcontra.
+       apply Wasm_int.Int32.repr_inv in Hcontra.
+       { by lias. }
+       { rewrite u32_modulus; unfold ffff0000 in Hvb; unfold two14 in Hlens; by lias. }
+       { rewrite u32_modulus; unfold ffff0000 in Hvb; unfold two14 in Hlens; by lias. }
+  }
+  { by iIntros "(%Habs & _)". }
+
+  iIntros (w) "(-> & Hf)" => /=.
+  rewrite separate2.
+  iApply wp_seq.
+  iSplitR; last iSplitL "Hf".
+  2: { iApply (wp_br_if_false with "Hf") => //=.
+       by instantiate (1 := λ w, ⌜ w = immV _ ⌝%I).
+  }
+  { by iIntros "(%Habs & _)". }
+
+  iIntros (w) "(-> & Hf)" => /=.
+  rewrite (separate1 (AI_basic _)).
+  iApply wp_seq.
+  iSplitR; last iSplitL "Hf".
+  2: { iApply wp_get_local => //.
+       by instantiate (1 := λ w, ⌜ w = immV _ ⌝%I).
+  }
+  { by iIntros "(%Habs & _)". }
+  
+  iIntros (w) "(-> & Hf)" => /=.
+  rewrite separate3.
+  iApply wp_seq.
+  iSplitR; last iSplitL "Hf".
+  2: { iApply (wp_binop with "Hf") => //=.
+       instantiate (1 := λ w, ⌜ w = immV [value_of_int (v + length s * 4 - 4 * j)]⌝%I) => /=.
+       iIntros "!>".
+       iPureIntro.
+       unfold value_of_int.
+       repeat f_equal.
+       unfold Wasm_int.Int32.iadd, Wasm_int.Int32.add => /=.
+       f_equal.
+       rewrite Wasm_int.Int32.Z_mod_modulus_eq.
+       rewrite Z.mod_small; last first.
+       { remember (length s) as x; rewrite - Heqx.
+         unfold ffff0000 in Hvb; rewrite u32_modulus; unfold two14 in Hlens.
+         lia.
+       }
+       lia.
+  }
+  { by iIntros "(%Habs & _)". }
+
+  iIntros (w) "(-> & Hf)" => /=.
+  rewrite separate2.
+  iApply wp_seq.
+  instantiate (1 := λ w, (⌜ w = immV [value_of_int (v+length s * 4 - 4 * j)] ⌝ ∗ ↪[frame] _)%I).
+  iSplitR; last iSplitL "Hf".
+  2: { iApply (wp_tee_local with "Hf").
+       iIntros "!> Hf".
+       rewrite (separate1 (AI_basic _)).
+       iApply wp_val_app => //.
+       iSplit; first by iIntros "!> (%Habs & _)" => /=.
+       iApply (wp_set_local with "[] [$Hf]"); first lia.
+       done.
+  }
+  { by iIntros "(%Habs & _)". }
+
+  iIntros (w) "(-> & Hf)" => /=.
+  rewrite separate2.
+  iApply wp_seq.
+  instantiate (1 := λ w, (⌜ w = immV [value_of_int (v+length s * 4 - 4 * j); value_of_int (v+length s * 4 - 4 * j)] ⌝ ∗ ↪[frame] _)%I).
+  iSplitR; last iSplitL "Hf".
+  2: { rewrite (separate1 (AI_basic _)).
+       iApply wp_val_app => //.
+       iSplit; first by iIntros "!> (%Habs & _)" => /=.
+       iApply (wp_get_local with "[] [$Hf]").
+       { rewrite - fmap_insert_set_nth => /=; last lia.
+         by rewrite list_lookup_insert; last lia.
+       }
+       done.
+  }
+  { by iIntros "(%Habs & _)". }
+
+  iIntros (w) "(-> & Hf)" => /=.
+  rewrite separate3.
+  iApply wp_seq.
+  instantiate (1 := λ w, (⌜ w = immV [value_of_int (v+length s * 4 - 4 * j); VAL_int32 sv] ⌝ ∗ isStack v s n ∗ ↪[frame] _)%I).
+  iSplitR; last iSplitL "Hf Hs".
+  2: { rewrite (separate1 (AI_basic _)).
+       iApply wp_val_app => //.
+       iSplit; first by iIntros "!> (%Habs & _)" => /=.
+       iApply (wp_wand with "[Hf Hs]").
+       { by iApply (stack_load_j with "[] [] [] [$Hs] [$Hf]") => //. }
+       iIntros (w) "(-> & Hs & Hf)" => /=.
+       iSplit => //.
+       by iFrame.
+  }
+  { by iIntros "(%Habs & _)". }
+  
+  iIntros (w) "(-> & Hs & Hf)" => /=.
+  rewrite separate3.
+  iApply wp_seq.
+  instantiate (1 := λ w, (⌜ w = immV [value_of_int (v+length s * 4 - 4 * j); VAL_int32 sv; VAL_int32 fn] ⌝ ∗ ↪[frame] _)%I).
+  iSplitR; last iSplitL "Hf".
+  2: { rewrite (separate2 (AI_basic _)).
+       iApply wp_val_app => //.
+       iSplit; first by iIntros "!> (%Habs & _)" => /=.
+       iApply (wp_get_local with "[] [$Hf]").
+       { rewrite - fmap_insert_set_nth => /=; last lia.
+         by rewrite list_lookup_insert_ne; last lia.
+       }
+       done.
+  }
+  { by iIntros "(%Habs & _)". }
+
+  iIntros (w) "(-> & Hf)" => /=.
+  rewrite separate4.
+  iApply wp_seq.
+  instantiate (1 := λ w, (∃ v0, ⌜ w = immV [value_of_int (v+length s * 4 - 4 * j); VAL_int32 v0] ⌝ ∗ Ψ sv v0 ∗ _)%I).
+  iSplitR; last iSplitL "Hf HΦ Htab Hcl".
+  2: { rewrite (separate1 (AI_basic _)).
+       iApply wp_val_app => //.
+       iSplit; first by iIntros "!> H" => /=; iDestruct "H" as (v0) "(%Habs & _)".
+       iApply (wp_call_indirect_success_ctx with "[$Htab] [$Hcl] [$Hf] [HΦ]") => /=.
+       { by rewrite Hclt. }
+       { done. }
+       2: { iPureIntro.
+            instantiate (1 := (LH_base [AI_basic (BI_const (VAL_int32 sv))] [])).
+            instantiate (1 := 0).
+            unfold lfilled, lfill.
+            simpl.
+            by apply/eqP.
+       }
+       { iIntros "!> (Htab & Hcl & Hf)".
+         iApply wp_base_pull.
+         iApply wp_wasm_empty_ctx.
+         iApply ("Hspec" with "[$HΦ $Htab $Hcl $Hf]"); first done.
+         iIntros (w) "(Hret & Hf & Htab & Hcl)".
+         iDestruct "Hret" as (v0) "(-> & HΨ)".
+         iExists v0.
+         iSplit => //.
+         iFrame "HΨ".
+         iCombine "Hf Htab Hcl" as "H".
+         by iApply "H".
+       }
+  }
+  { by iIntros "H"; iDestruct "H" as (v0) "(%Habs & _)". }
+
+  iIntros (w) "H".
+  iDestruct "H" as (v0) "(-> & HΨ & Hf & Htab & Hcl)" => /=.
+  rewrite separate3.
+  iApply wp_seq.
+  iSplitR; last iSplitL "Hf Hs".
+  2: { by iApply (stack_store_j with "[] [] [] [$Hs] [$Hf]") => //. }
+  { by iIntros "(%Habs & _)". }
+
+  iIntros (w) "(-> & Hs & Hf)" => /=.
+  iApply (wp_wand with "[Hf]").
+  { iApply wp_value; last iFrame.
+    { by instantiate (1 := brV (VH_base 0 [] [])). }
+    { by instantiate (1 := λ w, (⌜ w = brV _ ⌝ ∗ ↪[frame] _)%I); iFrame. }
+  }
+  
+  iIntros (w) "(-> & Hf)" => /=.
+  iApply "HΞ".
+  iSplit => //.
+  iSplitL "HΨ Hs"; first by iExists v0; iFrame.
+  iFrame.
+  by rewrite - fmap_insert_set_nth; last lia.
+Qed.
+
+Lemma spec_map_loop_j f (s: list i32) v n E j fn j0 a cl
+      (Φ : i32 -> iPropI Σ) (Ψ: i32 -> i32 -> iPropI Σ) (s': list i32):
+  ⊢ ( ⌜ f.(f_inst).(inst_memory) !! 0 = Some n ⌝ ∗
+        ⌜ f.(f_locs) !! 0 = Some (value_of_int v) ⌝ ∗
+        ⌜ f.(f_locs) !! 1 = Some (VAL_int32 fn) ⌝  ∗
+        ⌜ f.(f_locs) !! 2 = Some (value_of_int (v + (length s) * 4 - 4 * j)) ⌝ ∗
+        ⌜ f.(f_locs) !! 3 = Some (value_of_int (v + (length s) * 4)) ⌝ ∗
+        ⌜ length f.(f_locs) >= 4 ⌝ ∗
+        ⌜ (0 <= j <= length s)%Z ⌝ ∗
+        ⌜ (j + length s' = length s)%Z ⌝ ∗
+        isStack v (take (Z.to_nat j) s ++ s') n ∗
+        stackAll (take (Z.to_nat j) s) Φ ∗
+        stackAll2 (drop (Z.to_nat j) s) s' Ψ ∗
+            ⌜ f.(f_inst).(inst_types) !! 1 = Some (Tf [T_i32] [T_i32]) ⌝ ∗
+            ⌜ f.(f_inst).(inst_tab) !! 0 = Some j0 ⌝ ∗
+            (N.of_nat j0) ↦[wt][ N.of_nat (Wasm_int.nat_of_uint i32m fn) ] (Some a) ∗
+            (N.of_nat a) ↦[wf] cl ∗
+            ⌜ cl_type cl = Tf [T_i32] [T_i32] ⌝ ∗ 
+            (∀ (u : i32) (fc : frame),
+                {{{ Φ u ∗
+                      ⌜ f_inst f = f_inst fc ⌝ ∗
+                       ↪[frame] fc ∗
+                       (N.of_nat j0) ↦[wt][ N.of_nat (Wasm_int.nat_of_uint i32m fn) ] (Some a) ∗
+                       (N.of_nat a) ↦[wf] cl
+                  }}}
+                  [ AI_basic (BI_const (VAL_int32 u)) ;
+                    AI_invoke a ] @ E
+                  {{{ w, (∃ v, ⌜ w = immV [VAL_int32 v] ⌝ ∗ Ψ u v)
+                           ∗ ↪[frame] fc
+                           ∗ (N.of_nat j0) ↦[wt][ N.of_nat (Wasm_int.nat_of_uint i32m fn) ] (Some a) 
+                           ∗ (N.of_nat a) ↦[wf] cl }}}) ∗   
+            ↪[frame] f) -∗
+  WP (to_e_list map_loop_body) @ E CTX 2;
+  push_base (LH_rec [] 0 [] (LH_base [] []) []) 0
+    [AI_basic
+       (BI_loop (Tf [] [])
+          map_loop_body)] [] []
+    {{ w, ⌜ w = immV [] ⌝ ∗
+           (∃ s', isStack v s' n ∗ stackAll2 s s' Ψ) ∗
+           (∃ f1, ↪[frame] f1 ∗ ⌜ f_inst f = f_inst f1 ⌝) ∗
+            (N.of_nat j0) ↦[wt][ N.of_nat (Wasm_int.nat_of_uint i32m fn) ] (Some a) ∗
+            (N.of_nat a) ↦[wf] cl
+    }}.
+Proof.
+  remember (Z.to_nat j) as k.
+  iRevert (Heqk).
+  iRevert (j s' s f).
+  iInduction k as [|k] "IHk".
+  
+  { iIntros (j s' s f Habs).
+    iIntros "(%Hinstmem & %Hlocs0 & %Hlocs1 & %Hlocs2 & %Hlocs3 & %Hlocs & %Hjbound & %Hlen & Hs & HΦ & HΨ & %Htypes & %Htab & Htab & Hcl & %Hclt & #Hspec & Hf)" => /=.
+
+    iDestruct (stack_pure with "Hs") as "(%Hdiv & %Hvb & %Hlens & Hs)".
+    
+    assert (j=0)%Z as ->; first lia.
+    iApply wp_ctx_bind => //.
+    iApply (spec_map_loop_body_terminate with "[Hs Hf]").
+    { iFrame.
+      repeat iSplit => //.
+      iPureIntro.
+      lia.
+    }
+    iIntros (w) "(%Hes & Hs & Hf)".
+    destruct Hes as [es ->] => /=.
+    rewrite (separate1 (AI_basic _)).
+    replace ([AI_basic (BI_br 1)] ++ es) with ([] ++ [AI_basic (BI_br 1)] ++ es) => //.
+    iApply wp_base_push => //.
+    replace ([AI_basic (BI_br 1)]) with ([] ++ [AI_basic (BI_br 1)]) => //.
+    iApply (wp_br_ctx with "Hf") => //.
+    iIntros "!> Hf" => /=.
+    iApply wp_value; first by instantiate (1 := immV []).
+    iSplit => //.
+    iSplitL "HΨ Hs".
+    { iExists s'.
+      rewrite drop_0.
+      by iFrame.
+    }
+    iSplitL "Hf".
+    { by iExists f; iSplit => //. }
+    by iFrame.
+  }
+  
+  { iIntros (j s' s f Habs).
+    iIntros "(%Hinstmem & %Hlocs0 & %Hlocs1 & %Hlocs2 & %Hlocs3 & %Hlocs & %Hjbound & %Hlen & Hs & HΦ & HΨ & %Htypes & %Htab & Htab & Hcl & %Hclt & #Hspec & Hf)" => /=.
+    
+    iDestruct (stack_pure with "Hs") as "(%Hdiv & %Hvb & %Hlens & Hs)".
+
+    assert (j = Z.of_nat (k+1)) as ->; first lia.
+
+    assert (exists sv, s !! k = Some sv) as Hsvlookup.
+    { destruct (s !! k) eqn:Hol => //; first by eexists.
+      apply lookup_ge_None in Hol.
+      lia.
+    }
+    destruct Hsvlookup as [sv Hsvlookup].
+
+    assert (take (S k) s = take k s ++ [sv]) as HStake; first by erewrite take_S_r.
+    rewrite HStake.
+
+    iDestruct (stackAll_app with "HΦ") as "(HΦ & HsvΦ)".
+    simpl.
+    iDestruct "HsvΦ" as "(HsvΦ & _)".
+
+    rewrite - HStake.
+
+    iApply wp_ctx_bind => //.
+    iApply (spec_map_loop_body_continue with "[Hs HsvΦ Htab Hcl Hf]").
+    { iFrame.
+      repeat rewrite app_length take_length.
+      replace (S k `min` length s) with (S k); last lia.
+      replace (S k + length s') with (length s); last lia.
+      instantiate (6 := k).
+      repeat iSplit => //.
+      { rewrite Hlocs2.
+        iPureIntro.
+        do 2 f_equal.
+        lia.
+      }
+      { iPureIntro. lia. }
+      { iPureIntro. lia. }
+      { iPureIntro.
+        rewrite lookup_app.
+        replace (take _ _ !! Z.to_nat k) with (Some sv) => //.
+        rewrite lookup_take; last lia.
+        by rewrite Nat2Z.id.
+      }
+    }
+    
+    iIntros (w) "(-> & H)" => /=.
+
+    iDestruct "H" as "(HsvΨ & Htab & Hcl & Hf)".
+    iDestruct "HsvΨ" as (sv') "(Hs & HΨ')".
+    
+    replace ([AI_basic (BI_br 0)]) with ([] ++ [AI_basic (BI_br 0)]) => //.
+    iApply (wp_br_ctx_nested with "Hf") => //; first lia.
+    { by instantiate (1 := LH_rec [] 0 [] (LH_base [] []) []) => //=. }
+
+    iIntros "!> Hf".
+    rewrite - (app_nil_l [AI_basic (BI_loop _ _)]).
+    iApply (wp_loop_ctx with "Hf") => //.
+    iIntros "!> Hf".
+    replace (cat [] (to_e_list map_loop_body)) with ([] ++ to_e_list map_loop_body ++ []); last done.
+    iApply wp_label_push => //.
+    simpl.
+    remember ({| f_locs := <[2:=value_of_int (v + length (take (S k) s ++ s') * 4 - 4 * k)]> (f_locs f);
+                 f_inst := f_inst f |}) as f'.
+    rewrite -Heqf'.
+    replace (f_inst f) with (f_inst f'); last by rewrite Heqf'.
+
+    iApply "IHk"; first by iPureIntro; instantiate (1 := k); rewrite Nat2Z.id.
+    rewrite Heqf' => /=.
+    iCombine "HΨ HΨ'" as "HΨcomb".
+    iFrame.
+    instantiate (1 := (sv' :: s')).
+    rewrite app_length take_length.
+    assert (S k `min` length s = S k) as Hmin; first lia.
+    rewrite Hmin.
+    repeat iSplit => //.
+    { by rewrite list_lookup_insert_ne. }
+    { by rewrite list_lookup_insert_ne. }
+    { rewrite list_lookup_insert; last lia.
+      iPureIntro.
+      do 2 f_equal.
+      rewrite - Hlen.
+      by lias.
+    }
+    { by rewrite list_lookup_insert_ne. }
+    { rewrite insert_length. iPureIntro; lia. }
+    { iPureIntro. lia. }
+    { iPureIntro.
+      assert (k+1 <= length s)%Z as H; first lias. clear - H.
+      remember (length s) as x.
+      rewrite - Heqx.
+      lia.
+    }
+    { iPureIntro.
+      simpl.
+      clear - Hlen.
+      remember (length s) as x; rewrite - Heqx.
+      remember (length s') as x'; rewrite - Heqx'.
+      lia.
+    }
+    iSplitL "Hs".
+    { replace (<[_ := _]> _) with (take k s ++ sv' :: s'); first done.
+      erewrite take_S_r => //.
+      rewrite insert_app_l; last first.
+      { rewrite app_length take_length => /=.
+        remember (length s) as x.
+        rewrite - Heqx.
+        lia.
+      }
+      rewrite insert_app_r_alt; last first.
+      { rewrite take_length => /=.
+        remember (length s) as x.
+        rewrite - Heqx.
+        lia.
+      }
+      rewrite take_length.
+      remember (length s) as x.
+      rewrite - Heqx.
+      replace (k `min` x) with k; last lia.
+      replace (Z.to_nat k - k) with 0; last lia.
+      simpl.
+      rewrite - app_assoc.
+      done.
+    }
+    iSplitL "HΨcomb".
+    { assert ((drop k s) = (sv :: (drop (S k) s))) as Hdeq; first by erewrite drop_S.
+      rewrite Hdeq => /=.
+      by iDestruct "HΨcomb" as "(? & ?)"; iFrame.
+    }
+    by repeat iSplit => //.
+  }  
+Qed.
+  
 Lemma spec_stack_map (f0 : frame) (n : immediate) (f : i32) (v : Z) (s : seq.seq i32) E
       j0 a cl 
       (Φ : i32 -> iPropI Σ) (Ψ : i32 -> i32 -> iPropI Σ) :
   ⊢ {{{  ⌜ f0.(f_inst).(inst_memory) !! 0 = Some n ⌝  ∗
-            ⌜ f0.(f_locs) !! 0 = Some (VAL_int32 f) ⌝  ∗
-            ⌜ f0.(f_locs) !! 1 = Some (value_of_int v) ⌝ ∗
+            ⌜ f0.(f_locs) !! 0 = Some (value_of_int v) ⌝ ∗
+            ⌜ f0.(f_locs) !! 1 = Some (VAL_int32 f) ⌝  ∗
             ⌜ length f0.(f_locs) >= 4 ⌝ ∗
-            ⌜ (0 <= v)%Z ⌝ ∗                                   
-            ⌜ (v + 4 + length s * 4 ≤ Wasm_int.Int32.max_unsigned)%Z ⌝ ∗
             isStack v s n ∗
             stackAll s Φ ∗
             ⌜ f0.(f_inst).(inst_types) !! 1 = Some (Tf [T_i32] [T_i32]) ⌝ ∗
-
             ⌜ f0.(f_inst).(inst_tab) !! 0 = Some j0 ⌝ ∗
             (N.of_nat j0) ↦[wt][ N.of_nat (Wasm_int.nat_of_uint i32m f) ] (Some a) ∗
             (N.of_nat a) ↦[wf] cl ∗
-            ⌜ match cl with FC_func_native _ t _ _ => t | FC_func_host t _ => t end
-         = Tf [T_i32] [T_i32] ⌝ ∗ 
+            ⌜ cl_type cl = Tf [T_i32] [T_i32] ⌝ ∗ 
             (∀ (u : i32) (fc : frame),
                 {{{ Φ u ∗
                       ⌜ f_inst f0 = f_inst fc ⌝ ∗
@@ -99,93 +921,35 @@ Lemma spec_stack_map (f0 : frame) (n : immediate) (f : i32) (v : Z) (s : seq.seq
             (N.of_nat a) ↦[wf] cl
     }}}.
 Proof.
-  iIntros "!>" (Ξ) "(%Hinstmem & %Hlocs0 & %Hlocs1 & %Hlocs & %Hvb & %Hv & Hs & HΦ & %Htypes & %Htab & Htab & Hcl & %Hclt & #Hspec & Hf) HΞ" => /=.
+  iIntros "!>" (Ξ) "(%Hinstmem & %Hlocs0 & %Hlocs1 & %Hlocs & Hs & HΦ & %Htypes & %Htab & Htab & Hcl & %Hclt & #Hspec & Hf) HΞ" => /=.
+
   rewrite separate4.
   iApply wp_seq.
-  instantiate (1 := λ x,  (⌜ x = immV [] ⌝ ∗ isStack v s n ∗ ↪[frame] f0)%I).
-  iSplitR; first by iIntros "(%H & _)".
-  iSplitL "Hs Hf"; first by iApply (is_stack_valid with "[$Hs $Hf]").
-  iIntros (w) "(-> & Hs & Hf)".
-  simpl.
-  rewrite (separate1 (AI_basic (BI_get_local 1))).
-  iApply wp_seq.
-  iSplitR ; last first.
-  iSplitL "Hf".
-  iApply wp_get_local => //.
-  instantiate (1 := λ x, ⌜x = immV [value_of_int v]⌝%I) => //.
-  iIntros (w) "[-> Hf]".
-  iSimpl.
-  rewrite (separate2 (AI_basic (i32const v))).
-  iApply wp_seq.
-  iSplitR ; last first.
-  iSplitL "Hf Hs".
-  iApply wp_load => // ; last first.
-  unfold isStack.
-  iDestruct "Hs" as "(% & % & Hn & ?)".
-  iDestruct (i32_wms with "Hn") as "Hn".
-  rewrite N.add_0_r.
-  simpl.
-  rewrite Wasm_int.Int32.Z_mod_modulus_eq.
-  rewrite Z.mod_small.
-  unfold bits.
-  instantiate (1 := VAL_int32 _) => /=.
-  iFrame.
-  iNext.
-  instantiate ( 1 := λ x, (⌜ x = immV [value_of_int (v + 4 + length s * 4)] ⌝ ∗
-                                     ⌜(two16 | v)%Z⌝ ∗
-                                     ⌜(length s < two14)%Z⌝ ∗
-                                     ([∗ list] i↦w ∈ s, N.of_nat n ↦[i32][ Z.to_N (v + 4 + length s * 4 - 4 - 4 * i)] w) ∗
-      (∃ bs : seq.seq byte, ⌜Z.of_nat (length bs) = (two16 - 4 - length s * 4)%Z⌝ ∗
-                                                                              N.of_nat n↦[wms][Z.to_N (v + 4 + length s * 4)]bs))%I).
-  iFrame.
-  done.
-  unfold Wasm_int.Int32.max_unsigned in Hv ; lia.
-  done.
-  iIntros (w) "[[[-> Hs] Hn] Hf]".
-  iSimpl.
-  rewrite (separate2 (AI_basic (i32const (v + _ + _)))).
-  iApply wp_seq.
-  iSplitR ; last first.
-  iSplitL "Hf".
-  iApply wp_set_local => //.
-  by instantiate (1 := λ x, ⌜x = immV []⌝%I).
-  iIntros (w) "[-> Hf]".
-  iSimpl.
-  rewrite (separate1 (AI_basic (BI_get_local 1))).
-  iApply wp_seq.
-  iSplitR ; last first.
-  iSplitL "Hf".
-  iApply (wp_get_local with "[] [$Hf]") => //=.
-  unfold set_nth.
-  destruct (f_locs f0) ; first by inversion Hlocs0.
-  destruct l ; first by inversion Hlocs1.
-  simpl in Hlocs1.
-  inversion Hlocs1 ; subst.
-  done.
-  by instantiate (1 := λ x, ⌜x = immV [value_of_int v]⌝%I).
-  iIntros (w) "[-> Hf]".
-  iSimpl.
+  iSplitR; last iSplitL "Hf Hs".
+  2: { by iApply (is_stack_valid with "[$Hf $Hs]") => //. }
+  { by iIntros "(%Habs & _)". }
+
+  iIntros (w) "(-> & Hs & Hf)" => /=.
   rewrite separate3.
   iApply wp_seq.
-  iSplitR ; last first.
-  iSplitL "Hf".
-  iApply (wp_binop with "Hf") => //.
-  by instantiate (1 := λ x, ⌜ x = immV [_] ⌝%I).
-  iIntros (w) "[-> Hf]".
-  iSimpl.
-  rewrite (separate2 _ (AI_basic (BI_set_local 2))).
+  iSplitR; last iSplitL "Hf Hs".
+  2: { by iApply (is_stack_bound_valid with "[$Hf $Hs]") => //. }
+  { by iIntros "(%Habs & _)". }
+  
+  iIntros (w) "(-> & Hs & Hf)" => /=.
+  rewrite separate5.
   iApply wp_seq.
-  iSplitR ; last first.
-  iSplitL "Hf".
-  iApply wp_set_local => //=.
-  simpl.
-  rewrite length_is_size size_set_nth.
-  rewrite length_is_size in Hlocs.
-  unfold ssrnat.maxn.
-  destruct (ssrnat.leq _ _) ; lia.
-  by instantiate (1 := λ x, ⌜x = immV []⌝%I).
-  iIntros (w) "[-> Hf]".
-  iSimpl.
+  iSplitR; last iSplitL "Hf Hs".
+  2: { iApply (spec_map_initialise with "[$Hf $Hs]") => //.
+       iIntros (w) "(-> & Hs & Hf)".
+       instantiate (1 := λ w, (⌜w = immV []⌝ ∗ _)%I).
+       iSplit => //.
+       iCombine "Hs Hf" as "H".
+       by iApply "H".
+  }
+  { by iIntros "(%Habs & _)". }
+
+  iIntros (w) "(-> & Hs & Hf)" => /=.
   rewrite - (app_nil_l [AI_basic (BI_block _ _)]).
   iApply (wp_block with "Hf") => //.
   iIntros "!> Hf".
@@ -198,1663 +962,50 @@ Proof.
   iIntros "!> Hf".
   simpl.
   rewrite - (cat0s (AI_basic (BI_get_local 2) :: _)).
-  rewrite - (cats0 [AI_basic _;_;_;_;_;_;_;_;_;_;_;_;_;_;_]). 
+  rewrite - (cats0 [AI_basic _;_;_;_;_;_;_;_;_;_;_;_;_;_]). 
   iApply wp_label_push ; first done.
-  unfold Wasm_int.Int32.iadd, Wasm_int.Int32.add.
-  rewrite Wasm_int.Int32.unsigned_repr ; last lia.
-  rewrite Wasm_int.Int32.unsigned_repr ; last by unfold Wasm_int.Int32.max_unsigned,
-      Wasm_int.Int32.modulus, Wasm_int.Int32.wordsize, Integers.Wordsize_32.wordsize.
-  iAssert (∀ (j :nat) s', ⌜ j <= length s ⌝ -∗ ⌜ length s' = length s - j ⌝ -∗ ↪[frame] {|
-                    f_locs :=
-                      set_nth (VAL_int32 (Wasm_int.Int32.repr (v + 4 )))
-                        (set_nth
-                           (VAL_int32 (Wasm_int.Int32.repr (v + 4 + length s * 4)))
-                           (f_locs f0) 3
-                           (VAL_int32 (Wasm_int.Int32.repr (v + 4 + length s * 4)))) 2
-                        (VAL_int32 (Wasm_int.Int32.repr (v + 4 + (length s - j%Z) * 4)));
-                    f_inst := f_inst f0
-                    |} -∗
-                    isStack v (take j s ++ s') n -∗ 
-                    stackAll (take j s) Φ -∗
-                    stackAll2 (drop j s) s' Ψ -∗
-                    N.of_nat j0 ↦[wt][N.of_nat (Z.to_nat (Wasm_int.Int32.unsigned f))]Some a -∗
-                    N.of_nat a↦[wf] cl -∗
-                    (∀ w : val,
-                        ⌜w = immV []⌝ ∗ (∃ s' : seq.seq i32, isStack v s' n ∗ stackAll2 s s' Ψ) ∗
-                                  (∃ f1 : frame,  ↪[frame]f1 ∗ ⌜f_inst f0 = f_inst f1⌝) ∗
-              N.of_nat j0↦[wt][N.of_nat (Z.to_nat (Wasm_int.Int32.unsigned f))]
-              Some a ∗ N.of_nat a↦[wf]cl -∗ 
-                                  Ξ w) -∗
-                    WP [AI_basic (BI_get_local 2); AI_basic (BI_get_local 3);
-     AI_basic (BI_relop T_i32 (Relop_i (ROI_ge SX_U))); AI_basic (BI_br_if 1);
-     AI_basic (BI_get_local 2); AI_basic (BI_get_local 2); AI_basic (BI_get_local 2);
-     AI_basic (BI_load T_i32 None N.zero N.zero); AI_basic (BI_get_local 0);
-     AI_basic (BI_call_indirect 1); AI_basic (BI_store T_i32 None N.zero N.zero);
-     AI_basic (i32const 4); AI_basic (BI_binop T_i32 (Binop_i BOI_add));
-     AI_basic (BI_set_local 2); AI_basic (BI_br 0)] @  E
-  CTX
-  2;
-  push_base (LH_rec [] 0 [] (LH_base [] []) []) 0
-    [AI_basic
-       (BI_loop (Tf [] [])
-          [BI_get_local 2; BI_get_local 3; BI_relop T_i32 (Relop_i (ROI_ge SX_U));
-          BI_br_if 1; BI_get_local 2; BI_get_local 2; BI_get_local 2;
-          BI_load T_i32 None N.zero N.zero; BI_get_local 0; 
-          BI_call_indirect 1; BI_store T_i32 None N.zero N.zero; 
-          i32const 4; BI_binop T_i32 (Binop_i BOI_add); BI_set_local 2; 
-          BI_br 0])] [] []
-    {{ v0, Ξ v0 }})%I as "H".
-  { iIntros (j).
-    iInduction j as [|j] "IHj".
-  { iIntros (s') "%Hj %Hs' Hf Hs HΦ HΨ Htab Hcl HΞ".
-    rewrite (separate1 (AI_basic (BI_get_local 2))).
-    iApply wp_seq_ctx.
-    iSplitR ; last first.
-    iSplitL "Hf".
-    iApply (wp_get_local with "[] [$Hf]").
-    simpl. by rewrite set_nth_read.
-    by instantiate ( 1 := λ x, ⌜x = immV _⌝%I).
-    iIntros (w) "[-> Hf]".
-    iSimpl.
-    rewrite (separate2 _ (AI_basic (BI_get_local 3))).
-    iApply wp_seq_ctx.
-    iSplitR ; last first.
-    iSplitL "Hf".
-    rewrite (separate1 _ [AI_basic (BI_get_local 3)]).
-    iApply wp_val_app => //.
-    iSplitR ; last first.
-    iApply wp_wand_r.
-    iSplitL.
-    iApply (wp_get_local with "[] [$Hf]").
-    simpl.
-    destruct (f_locs f0) ; first by inversion Hlocs.
-    destruct l ; first by inversion Hlocs1.
-    destruct l ; first by simpl in Hlocs ; lia.
-    simpl.
-    by rewrite set_nth_read.
-    by instantiate (1 := λ x, ⌜x = immV _⌝%I).
-    iIntros (w) "[-> Hf]".
-    rewrite Z.sub_0_r.
-    iSimpl.
-    instantiate (1 := λ x, (⌜ x = immV _ ⌝ ∗ ↪[frame] _)%I).
-    iFrame.
-    done.
-    by iIntros "!> [% _]".
-    iIntros (w) "[-> Hf]".
-    iSimpl.
-    rewrite (separate3 _ _ (AI_basic (BI_relop _ _))).
-    iApply wp_seq_ctx.
-    iSplitR ; last first.
-    iSplitL "Hf".
-    iApply (wp_relop with "Hf").
-    simpl.
-    unfold Wasm_int.Int32.ltu.
-    rewrite Wasm_int.Int32.unsigned_repr.
-    rewrite Coqlib.zlt_false.
-    simpl.
-    done.
-    lia.
-    split ; try lia.
-    exact Hv.
-    by instantiate (1 := λ x, ⌜ x = immV _ ⌝%I).
-    iIntros (w) "[-> Hf]".
-    iSimpl.
-    rewrite - (app_nil_l (AI_basic (i32const 1) :: _)).
-    rewrite (separate2 _ (AI_basic (BI_br_if 1))).
-    iApply wp_base_push ; first done.
-    iApply (wp_br_if_true_ctx with "Hf").
-    done.
-    iIntros "!> Hf".
-    rewrite - (app_nil_l [AI_basic (BI_br 1)]).
-    iApply (wp_br_ctx with "Hf") => //.
-    iIntros "!> Hf".
-    iApply wp_value.
-    unfold IntoVal.
-    by apply of_to_val.
-    iApply "HΞ".
-    iSplit ; first done.
-    iFrame. iSplitR "Hf".
-    iExists s'.
-    unfold take.
-    unfold drop.
-    iFrame.
-    iExists _.
-    iFrame.
-    done.
-    all : try by iIntros "[% _]". }
-  iIntros (s') "%Hj %Hs' Hf Hs HΦ HΨ Htab Hcl HΞ".
-  destruct s as [|v0 s]; first by inversion Hj.
-  cut (exists ys y, v0 :: take j s = ys ++ [y]) ;
-  [ intro Htail ; destruct Htail as (ys & y & Htail) |
-    exists (removelast (v0 :: take j s)) ;
-    exists (List.last (v0 :: take j s) (Wasm_int.Int32.repr 1)) ;
-    apply app_removelast_last ;
-    apply not_eq_sym ; apply nil_cons ].
-  simpl in Hv.
-  simpl in Hj.
-  assert (j `min` length s = j) as Hjmin.
-  { remember (length s) as x. rewrite - Heqx in Hj.
-    lia. } 
-  rewrite (separate1 (AI_basic (BI_get_local 2))).
-  iApply wp_seq_ctx.
-  iSplitR ; last first.
-  iSplitL "Hf".
-  iApply (wp_get_local with "[] [$Hf]").
-  simpl. by rewrite set_nth_read.
-  by instantiate ( 1 := λ x, ⌜x = immV _⌝%I).
-  iIntros (w) "[-> Hf]".
-  iSimpl.
-  rewrite (separate2 _ (AI_basic (BI_get_local 3))).
-  iApply wp_seq_ctx.
-  iSplitR ; last first.
-  iSplitL "Hf".
-  rewrite (separate1 _ [AI_basic (BI_get_local 3)]).
-  iApply wp_val_app => //.
-  iSplitR ; last first.
-  iApply wp_wand_r.
-  iSplitL.
-  iApply (wp_get_local with "[] [$Hf]").
-  simpl.
-  destruct (f_locs f0) ; first by inversion Hlocs.
-  destruct l ; first by inversion Hlocs1.
-  destruct l ; first by simpl in Hlocs ; lia.
-  simpl.
-  by rewrite set_nth_read.
-  by instantiate (1 := λ x, ⌜x = immV _⌝%I).
-  iIntros (w) "[-> Hf]".
-  iSimpl.
-  instantiate (1 := λ x, (⌜ x = immV _ ⌝ ∗ ↪[frame] _)%I).
-  iFrame.
-  done.
-  by iIntros "!> [% _]".
-  iIntros (w) "[-> Hf]".
-  iSimpl.
-  rewrite (separate3 _ _ (AI_basic (BI_relop _ _))).
-  iApply wp_seq_ctx.
-  iSplitR ; last first.
-  iSplitL "Hf".
-  iApply (wp_relop with "Hf").
-  simpl.
-  unfold Wasm_int.Int32.ltu.
-  rewrite Wasm_int.Int32.unsigned_repr.
-  rewrite Wasm_int.Int32.unsigned_repr.
-  rewrite Coqlib.zlt_true.
-  simpl.
-  done.
-  lia.
-  lia.
-  lia.
-  by instantiate (1 := λ x, ⌜ x = immV _ ⌝%I).
-  iIntros (w) "[-> Hf]".
-  iSimpl.
-  rewrite (separate2 (AI_basic (BI_const (VAL_int32 _)))).
-  iApply wp_seq_ctx.
-  iSplitR ; last first.
-  iSplitL "Hf".
-  iApply (wp_br_if_false with "Hf").
-  done.
-  iNext.
-  by instantiate (1 := λ x, ⌜ x = immV [] ⌝%I).
-  iIntros (w) "[-> Hf]".
-  iSimpl.
-  rewrite (separate1 (AI_basic (BI_get_local 2)) [_;_;_;_;_;_;_;_;_;_]).
-  iApply wp_seq_ctx.
-  iSplitR ; last first.
-  iSplitL "Hf".
-  iApply (wp_get_local with "[] [$Hf]") => /=.
-  by rewrite set_nth_read.
-  by instantiate (1 := λ x, ⌜x = immV _⌝%I).
-  iIntros (w) "[-> Hf]".
-  iSimpl.
-  rewrite (separate2 (AI_basic (i32const (v + 4 + _ * 4)))).
-  iApply wp_seq_ctx.
-  iSplitR ; last first.
-  iSplitL "Hf".
-  rewrite (separate1 (AI_basic (i32const (v + 4 + _ * 4)))).
-  iApply wp_val_app. done.
-  iSplitR ; last first.
-  iApply wp_wand_r.
-  iSplitL.
-  iApply (wp_get_local with "[] [$Hf]") => /=.
-  by rewrite set_nth_read.
-  by instantiate (1 := λ x, ⌜x = immV _⌝%I).
-  iIntros (w) "[-> Hf]".
-  iSimpl.
-  by instantiate (1 := λ x, (⌜ x = immV _ ⌝ ∗ ↪[frame] _)%I) ; iFrame.
-  by iIntros "!> [% _]".
-  iIntros (w) "[-> Hf]".
-  iSimpl.
-  rewrite (separate3 (AI_basic (i32const (v + 4 + _ * 4)))).
-  iApply wp_seq_ctx.
-  iSplitR ; last first.
-  iSplitL "Hf".
-  rewrite (separate2 (AI_basic (i32const (v + 4 + _ * 4)))).
-  iApply wp_val_app ; first done.
-  iSplitR ; last first.
-  iApply wp_wand_r.
-  iSplitL.
-  iApply (wp_get_local with "[] [$Hf]") => /=.
-  by rewrite set_nth_read.
-  by instantiate (1 := λ x, ⌜x = immV _⌝%I).
-  iIntros (w) "[-> Hf]".
-  iSimpl.
-  by instantiate (1 := λ x, (⌜ x = immV _ ⌝ ∗ ↪[frame] _)%I) ; iFrame.
-  by iIntros "!> [% _]".
-  iIntros (w) "[-> Hf]".
-  iSimpl.
-  rewrite (separate4 (AI_basic (i32const (v + 4 + _ * 4)))).
-  iApply wp_seq_ctx.
-  iSplitR ; last first.
-  iSplitL "Hf Hs".
-  rewrite (separate2 (AI_basic (i32const (v + 4 + _ * 4)))).
-  iApply wp_val_app ; first done.
-  iSplitR ; last first.
- 
-  iApply wp_wand_r.
-  iSplitL.
 
-  iApply wp_load ; last first.
-  iFrame.
-  unfold isStack.
-  iDestruct "Hs" as "(Hdiv & Hlen & Hn & Hl & Hbs)".
-  rewrite cat_app.
-  iDestruct (big_sepL_app with "Hl") as "[Hs Hs']".
-  rewrite app_length.
-  rewrite Hs'.
-  rewrite take_length.
-  replace (S j `min` length (v0 :: s)) with (S j) ; last by simpl ; lia.
-  unfold take ; fold (take (A := value)).
-  rewrite Htail.
-  iDestruct (big_sepL_app with "Hs") as "[Hs H]".
-  iDestruct "H" as "[H _]".
-  iDestruct (i32_wms with "H") as "H" => //.
-  rewrite Nat.add_0_r.
-  rewrite N.add_0_r.
-  replace (Wasm_int.N_of_uint i32m (Wasm_int.Int32.repr (v + 4 + (S (length s) - S j) * 4)))
-    with (Z.to_N (v + 4 + (S (length s) - S j) * 4)).
-  replace (S j + (length (v0 :: s) - S j)) with (length (v0 :: s)) ; last by simpl ; lia.
-  replace (v + 4 + length (v0 :: s) * 4 - 4 - 4 * length ys)%Z
-    with (v + 4 + length (v0 :: s) * 4 - S (length ys) * 4)%Z ; last lia.
-  replace (S (length ys)) with (length (ys ++ [y])) ;
-    last by rewrite app_length ; simpl ; lia.
-  rewrite (cat_app ys [y]).
-  rewrite - Htail.
-  simpl.
-  rewrite firstn_length.
-  rewrite Hjmin.
-  rewrite (Z.mul_sub_distr_r (S (length s)) (S j) 4).
-  simpl in Hj.
-  remember (length s) as x.
-  rewrite - Heqx.
-  replace (v + 4 + S x * 4 - S j * 4)%Z
-    with (v + 4 + (S x * 4 - S j * 4))%Z ;
-    last lia.
-  rewrite Wasm_int.Int32.Z_mod_modulus_eq Z.mod_small.
-  instantiate (1 := VAL_int32 _).
-  iSplitR "H" ; last iExact "H".
-  iNext.
-  subst x.
-  instantiate ( 1 := λ x, (⌜ x = immV [VAL_int32 y] ⌝ ∗ ⌜ (two16 | v)%Z ⌝ ∗ ⌜ (S (length s) < two14)%Z ⌝ ∗ N.of_nat n ↦[i32][ Z.to_N v] Wasm_int.Int32.repr (v + 4 + S (length s) * 4) ∗  (∃ bs : seq.seq byte, ⌜ Z.of_nat (length bs) = (two16 - 4 - S (length s) * 4)%Z⌝ ∗
-            N.of_nat n↦[wms][Z.to_N (v + 4 + S (length s) * 4)]bs) ∗ ([∗ list] k↦y0 ∈ s', N.of_nat n
-                              ↦[i32][ Z.to_N
-                                        (v + 4 + S (length s) * 4 - 4 - 4 * S (j + k))] y0) ∗ [∗ list] k↦y0 ∈ ys, N.of_nat n
-                             ↦[i32][ Z.to_N (v + 4 + S (length s) * 4 - 4 - 4 * k)] y0)%I).
-  iFrame.
-  done.
-  simpl.
-  unfold Wasm_int.Int32.max_unsigned in Hv ; rewrite - Heqx in Hv ; lia.
-  simpl.
-  rewrite Wasm_int.Int32.Z_mod_modulus_eq.
-  rewrite Z.mod_small.
-  done.
-  unfold Wasm_int.Int32.max_unsigned in Hv ; lia.
-  done.
-  done.
-  iIntros (w) "[[[-> H1] H2] Hf]".
-  iSimpl.
-  instantiate (1 := λ x, (⌜ x = immV _ ⌝ ∗
-                                     ( ⌜(two16 | v)%Z⌝ ∗ ⌜(S (length s) < two14)%Z⌝ ∗ N.of_nat n ↦[i32][ Z.to_N v] Wasm_int.Int32.repr (v + 4 + S (length s) * 4) ∗
-         (∃ bs : seq.seq byte, ⌜Z.of_nat (length bs) = (two16 - 4 - S (length s) * 4)%Z⌝ ∗
-            N.of_nat n↦[wms][Z.to_N (v + 4 + S (length s) * 4)]bs) ∗
-         ([∗ list] k↦y0 ∈ s', N.of_nat n
-                              ↦[i32][ Z.to_N
-                                        (v + 4 + S (length s) * 4 - 4 - 4 * S (j + k))] y0) ∗
-         ([∗ list] k↦y0 ∈ ys, N.of_nat n
-                                       ↦[i32][ Z.to_N (v + 4 + S (length s) * 4 - 4 - 4 * k)] y0))
-                                     ∗ N.of_nat n↦[wms][Wasm_int.N_of_uint i32m
-                            (Wasm_int.Int32.repr (v + 4 + (length (v0 :: s) - S j) * 4)) +
-                                                          N.zero]bits (VAL_int32 y)
-                                     ∗ ↪[frame] {|
-                    f_locs :=
-                      set_nth
-                        (VAL_int32
-                           (Wasm_int.Int32.repr (v + 4)))
-                        (set_nth
-                           (VAL_int32
-                              (Wasm_int.Int32.repr (v + 4 + length (v0 :: s) * 4)))
-                           (f_locs f0) 3
-                           (VAL_int32
-                              (Wasm_int.Int32.repr (v + 4 + length (v0 :: s) * 4)))) 2
-                        (VAL_int32
-                           (Wasm_int.Int32.repr (v + 4 + (length (v0 :: s) - S j) * 4)));
-                    f_inst := f_inst f0
-                                     |})%I).
-  iFrame.
-  done.
-  by iIntros "!> [% _]".
-  iIntros (w) "(-> & (Hdiv & Hlen & Hv & Hbs & Hs' & Hs) & H & Hf)".
-  iSimpl.
-  rewrite (separate4 (AI_basic (i32const (v + 4 + _ * 4)))).
-  iApply wp_seq_ctx.
-  iSplitR ; last first.
-  iSplitL "Hf".
-  rewrite (separate3 (AI_basic (i32const (v + 4 + _ * 4)))).
-  iApply wp_val_app ; first done.
-  iSplitR ; last first.
-  iApply wp_wand_r.
-  iSplitL.
-  iApply (wp_get_local with "[] [$Hf]") => /=.
-  destruct (f_locs f0) ; inversion Hlocs0.
-  simpl. done.
-  by instantiate (1 := λ x, ⌜x = immV _⌝%I).
-  iIntros (w) "[-> Hf]".
-  iSimpl.
-  by instantiate (1 := λ x, (⌜ x = immV _ ⌝ ∗ ↪[frame] _)%I) ; iFrame.
-  by iIntros "!> [% _]".
-  iIntros (w) "[-> Hf]".
-  iSimpl.
-  rewrite (separate5 (AI_basic (i32const (v + 4 + _ * 4)))).
-  iApply wp_seq_ctx.
-  iSplitR ; last first.
-  iSplitL "HΦ Hf Htab Hcl".
-  rewrite (separate2 (AI_basic (i32const (v + 4 + _ * 4)))).
-  iApply wp_val_app ; first done.
-  iSplitR ; last first.
-  iApply wp_wand_r ; iSplitL.
-  unfold take ; fold (take (A := value)).
-  rewrite Htail.
-  iDestruct (stackAll_app with "HΦ") as "(HΦ & Hy & _)".
-  rewrite (separate1 _ [_;AI_basic (BI_call_indirect 1)]).
-  rewrite - (app_nil_r [_ ; AI_basic (BI_call_indirect 1)]).
-  iApply wp_wasm_empty_ctx.
-  iApply wp_base_push ; first done.
-  iApply (wp_call_indirect_success_ctx with "Htab Hcl Hf").
-  simpl.
-  unfold cl_type.
-  rewrite Hclt.
-  done.
-  simpl.
-  done.
-  iIntros "!> (Htab & Hcl & Hf)".
-  iApply wp_base_pull.
-  iApply wp_wasm_empty_ctx.
-  simpl.
-  iApply ("Hspec" with "[Hy Hf Htab Hcl]").
-  iFrame.
-  iPureIntro => //=.
-  iIntros (w) "(H & Hf & ?)".
-  iDestruct "H" as (v1) "[-> Hv1]".
-  instantiate (1 := λ x, ((∃ v1, ⌜ x = immV _ ⌝ ∗ stackAll ys Φ ∗ Ψ y v1 ∗
-                         N.of_nat j0↦[wt][N.of_nat (Z.to_nat (Wasm_int.Int32.unsigned f))]
-                         Some a ∗
-                         N.of_nat a↦[wf]cl)∗ ↪[frame] _)%I) ;
+  iApply (wp_wand_ctx with "[HΦ Htab Hcl Hs Hf]").
+  { iApply spec_map_loop_j.
     iFrame.
-  iExists  _; by iFrame.
-  iIntros (w) "[H Hf]".
-  iDestruct "H" as (v1) "[-> H]".
-  iSimpl.
-  instantiate (1 := λ x, (∃ v1, ⌜ x = immV _ ⌝ ∗ stackAll ys Φ ∗ Ψ y v1 ∗
-                                           N.of_nat j0↦[wt][N.of_nat (Z.to_nat (Wasm_int.Int32.unsigned f))]
-                                            Some a ∗ N.of_nat a↦[wf]cl
-                                           ∗ ↪[frame] _)%I).
-  iExists _ ; by iFrame.
-  iIntros "!> H".
-  by iDestruct "H" as (v1) "[% _]".
-  iIntros (w) "Hf".
-  iDestruct "Hf" as (v1) "(-> & HΦ & Hv1 & Htab & Hcl & Hf)".
-  iSimpl.
-  rewrite (separate4 (AI_basic (i32const (v + 4 + _ * 4)))).
-  iApply wp_seq_ctx.
-  iSplitR ; last first.
-  iSplitL "Hf H".
-  rewrite (separate1 (AI_basic (i32const (v + 4 + _ * 4)))).
-  iApply wp_val_app ; first done.
-  iSplitR ; last first.
-  iApply wp_wand_r.
-  iSplitL.
-  iApply wp_store ; last first.
-  simpl.
-  iFrame.
-  iNext.
-  by instantiate (1 := λ x, ⌜ x = immV [] ⌝%I).
+    repeat iSplit => /=.
+    { done. }
+    { rewrite list_lookup_insert_ne; last lia.
+      rewrite list_lookup_insert_ne; last lia.
+      by rewrite Hlocs0.
+    }
+    { rewrite list_lookup_insert_ne; last lia.
+      rewrite list_lookup_insert_ne; last lia.
+      by rewrite Hlocs1.
+    }
+    { rewrite list_lookup_insert; last by rewrite insert_length; lia.
+      instantiate (1 := (length s)).
+      instantiate (1 := s).
+      simpl.
+      iPureIntro.
+      do 2 f_equal.
+      lia.
+    }
+    { rewrite list_lookup_insert_ne; last lia.
+      rewrite list_lookup_insert; last lia.
+      done.
+    }
+    { by repeat rewrite insert_length. }
+    { iPureIntro. lia. }
+    { done. }
+    { instantiate (1 := []) => /=.
+      iPureIntro. lia. }
+    { rewrite Nat2Z.id.
+      rewrite firstn_all cats0.
+      iFrame.
+      rewrite drop_all.
+      instantiate (1 := Ψ).
+      by repeat iSplit => //.
+    }
+  }
   done.
-  done.
-  done.
-  iIntros (w) "[[-> H] Hf]".
-  iSimpl.
-  by instantiate (1 := λ x, (⌜ x = immV _ ⌝ ∗ N.of_nat n↦[wms][ _ ] _ ∗ ↪[frame] _)%I) ;
-  iFrame.
-  by iIntros "!> [% _]".
-  iIntros (w) "(-> & H & Hf)".
-  iSimpl.
-  rewrite (separate3 (AI_basic (i32const (v + 4 + _ * 4)))).
-  iApply wp_seq_ctx.
-  iSplitR ; last first.
-  iSplitL "Hf".
-  iApply (wp_binop with "Hf").
-  done.
-  by instantiate (1 := λ x, ⌜ x = immV _ ⌝%I).
-  iIntros (w) "[-> Hf]".
-  iSimpl.
-  rewrite (separate2 (AI_basic (BI_const (VAL_int32 (Wasm_int.Int32.iadd _ _))))).
-  iApply wp_seq_ctx.
-  iSplitR ; last first.
-  iSplitL "Hf".
-  iApply (wp_set_local with "[] [$Hf]") => /=.
-  destruct (f_locs f0) ; first done.
-  destruct l ; first done.
-  destruct l ; first by simpl in Hlocs ; lia.
-  destruct l ; first by simpl in Hlocs ; lia.
-  simpl.
-  lia.
-  by instantiate (1 := λ x, ⌜x = immV _⌝%I).
-  iIntros (w) "[-> Hf]".
-  simpl.
-  rewrite set_nth_write.
-  all : try by iIntros "[% _]".
-  all : try by iIntros "Habs" ; iDestruct "Habs" as (?) "[% _]".
-  rewrite - (app_nil_l [AI_basic (BI_br 0)]).
-  iApply (wp_br_ctx_nested with "Hf").
-  lia.
-  done.
-  instantiate (1 := LH_rec [] 0 [] (LH_base [] []) []) => //=.
-  done.
-  done.
-  iIntros "!> Hf".
-  iSimpl.
-  rewrite - (app_nil_l [AI_basic (BI_loop _ _)]).
-  iApply (wp_loop_ctx with "Hf") => //.
-  iIntros "!> Hf".
-  simpl.
-  rewrite - (cat0s (AI_basic (BI_get_local 2) :: _)).
-  rewrite - (cats0 [AI_basic _;_;_;_;_;_;_;_;_;_;_;_;_;_;_]). 
-  iApply wp_label_push ; first done.
-  iApply ("IHj" with "[] [] [Hf] [Hv Hbs Hs' Hs H Hlen Hdiv] [HΦ] [HΨ Hv1] Htab Hcl").
-  iPureIntro.
-  lia.
-  instantiate (1 := v1 :: s').
-  iPureIntro.
-  simpl.
-  rewrite Hs' => //=.
-  lia.
-  unfold Wasm_int.Int32.iadd, Wasm_int.Int32.add.
-  rewrite Wasm_int.Int32.unsigned_repr.
-  rewrite Wasm_int.Int32.unsigned_repr.
-  remember (length s) as x. rewrite - Heqx.
-  replace (v + 4 + (S x - S j) * 4 + 4)%Z
-    with (v + 4 + (S x - j) * 4)%Z.
-  iExact "Hf".
-  lia.
-  lia.
-  lia.
-  unfold isStack.
-  iFrame.
-  iDestruct "Hlen" as "%".
-  iSplit ; first iPureIntro.
-  rewrite app_length.
-  rewrite firstn_length.
-  replace (j `min` length (v0 :: s)) with j ; last by simpl ; lia.
-  simpl.
-  rewrite Hs'.
-  simpl.
-  lia.
-  iSplitL "Hv".
-  rewrite app_length.
-  rewrite firstn_length.
-  simpl.
-  remember (length s) as x. rewrite - Heqx.
-  replace (j `min` S x) with j ; last by simpl ; lia.
-  simpl.
-  rewrite Hs'.
-  simpl.
-  rewrite - Heqx.
-  replace (j + S (x - j)) with (S (x)) ; last lia.
-  iExact "Hv".
-  iSplitR "Hbs".
-  iApply big_sepL_app.
-  iSplitL "Hs".
-  replace j with (j `min` S j) ; last lia.
-  rewrite - take_take.
-  simpl.
-  rewrite Htail.
-  replace j with (length ys).
-  rewrite take_app.
-  iApply (big_sepL_impl with "Hs").
-  iIntros "!>" (k x) "% H".
-  remember (length s) as z ; rewrite - Heqz.
-  replace (S z) with (length (ys ++ v1 :: s')) ; first done.
-  rewrite app_length.
-  simpl.
-  rewrite Hs'.
-  simpl.
-  rewrite - Heqz.
-  remember (length ys) as zz ; rewrite - Heqzz.
-  replace zz with j ; first lia.
-  specialize (f_equal length Htail) as Hl.
-  simpl in Hl.
-  rewrite app_length in Hl ; simpl in Hl.
-  rewrite firstn_length in Hl.
-  subst z. rewrite Hjmin in Hl. rewrite - Heqzz in Hl. lia.
-  specialize (f_equal length Htail) as Hl.
-  simpl in Hl.
-  rewrite app_length in Hl ; simpl in Hl.
-  rewrite firstn_length in Hl.
-  rewrite Hjmin in Hl.
-  remember (length ys) as zz.
-  rewrite - Heqzz in Hl.
-  lia.
-  iSplitL "H".
-  iApply i32_wms.
-  rewrite Wasm_int.Int32.Z_mod_modulus_eq.
-  rewrite Z.mod_small.
-  rewrite N.add_0_r.
-  rewrite Nat.add_0_r.
-  rewrite app_length.
-  rewrite firstn_length.
-  simpl.
-  remember (length s) as x ; rewrite - Heqx.
-  replace (j `min` S x) with j ; last by simpl ; lia.
-  rewrite Hs'.
-  simpl.
-  rewrite - Heqx.
-  replace (j + S (x - j)) with (S (x)) ; last lia.
-  replace (v + 4 + S x *4 - 4 -4 * j)%Z
-    with  (v + 4 + ( S x - S j) * 4)%Z ; last lia.
-  iExact "H".
-  unfold Wasm_int.Int32.max_unsigned in Hv.
-  lia.
-  iApply (big_sepL_impl with "Hs'").
-  iIntros "!>" (k x) "% H".
-  rewrite app_length.
-  rewrite firstn_length.
-  simpl.
-  remember (length s) as z ; rewrite - Heqz.
-  replace (j `min` S z) with j ; last by simpl ; lia.  
-  rewrite Hs'.
-  simpl.
-  rewrite - Heqz.
-  replace (j + S (z - j)) with (S z) ; last lia.
-  replace (S ( j + k)) with (j + S k) ; last lia.
-  iExact "H".
-  iDestruct "Hbs" as (bs) "[% H]".
-  iExists bs.
-  iSplit ; first iPureIntro.
-  rewrite app_length.
-  rewrite firstn_length.
-  simpl.
-  remember (length s) as x ; rewrite - Heqx.
-  replace (j `min` S x) with j ; last by simpl ; lia.
-  simpl.
-  rewrite Hs'.
-  simpl.
-  lia.
-  rewrite app_length.
-  rewrite firstn_length.
-  simpl.
-  remember (length s) as x ; rewrite - Heqx.
-  replace (j `min` S x) with j ; last by simpl ; lia.
-  simpl.
-  rewrite Hs'.
-  simpl.
-  rewrite - Heqx.
-  replace (j + S (x - j)) with (S x) ; last lia.
-  iExact "H".
-  replace j with (j `min` S j) ; last lia.
-  rewrite - take_take.
-  simpl.
-  rewrite Htail.
-  replace j with (length ys).
-  rewrite take_app.
-  done.
-  specialize (f_equal length Htail) as Hl.
-  simpl in Hl.
-  rewrite app_length in Hl ; simpl in Hl.
-  rewrite firstn_length in Hl.
-  rewrite Hjmin in Hl.
-  remember (length ys) as zz ; rewrite - Heqzz in Hl ;
-    lia.
-  rewrite - (take_drop j s).
-  rewrite app_comm_cons.
-  rewrite Htail.
-  rewrite take_drop.
-  rewrite drop_app_le.
-  replace j with (length ys).
-  rewrite drop_app.
-  simpl.
-  iFrame.
-  specialize (f_equal length Htail) as Hl.
-  simpl in Hl.
-  rewrite app_length in Hl ; simpl in Hl.
-  rewrite firstn_length in Hl.
-   rewrite Hjmin in Hl.
-  remember (length ys) as zz ; rewrite - Heqzz in Hl ;
-    lia.
-  specialize (f_equal length Htail) as Hl.
-  simpl in Hl.
-  rewrite app_length in Hl ; simpl in Hl.
-  rewrite firstn_length in Hl.
-  rewrite app_length.
-  rewrite - Hl.
-  lia.
-  iExact "HΞ". }
-  iApply ("H" with "[] [] [Hf] [Hn Hs] [HΦ] [] Htab Hcl").
-  instantiate (1 := length s).
-  iPureIntro ; lia.
-  instantiate (1 := []).
-  iPureIntro ; simpl ; lia.
-  rewrite Z.sub_diag.
-  rewrite Z.mul_0_l.
-  rewrite Z.add_0_r.
-  done.
-  iDestruct "Hs" as "(% & % & Hs & Hbs)".
-  iSplit ; first done.
-  iSplit ; first iPureIntro.
-  rewrite cats0 firstn_length.
-  rewrite Nat.min_id.
-  exact H0.
-  iSplitL "Hn".
-  iApply i32_wms.
-  rewrite N.add_0_r.
-  rewrite Wasm_int.Int32.Z_mod_modulus_eq.
-  rewrite Z.mod_small.
-  rewrite cats0 firstn_length.
-  rewrite Nat.min_id.
-  done.
-  unfold Wasm_int.Int32.max_unsigned in Hv ; lia.
-  iSplitL "Hs".
-  rewrite cats0 firstn_length.
-  rewrite firstn_all.
-  rewrite Nat.min_id.
-  done.
-  rewrite cats0 firstn_length.
-  rewrite Nat.min_id.
-  done.
-  rewrite firstn_all.
-  done.
-  rewrite drop_all.
-  done.
-  done.
-  all : try by iIntros "[% _]".
-  by iIntros "[[[% _] _] _]".
 Qed.
 
-
-
-Lemma spec_stack_map_trap `{!logrel_na_invs Σ} (f0 : frame) (n : immediate) (f : i32) (v : Z) (s : seq.seq i32) E
-      j0 a cl γ 
-      (Φ : i32 -> iPropI Σ) (Ψ : i32 -> i32 -> iPropI Σ) :
-  ↑γ ⊆ E ->
-  ⊢ {{{  ⌜ f0.(f_inst).(inst_memory) !! 0 = Some n ⌝  ∗
-            ⌜ f0.(f_locs) !! 0 = Some (VAL_int32 f) ⌝  ∗
-            ⌜ f0.(f_locs) !! 1 = Some (value_of_int v) ⌝ ∗
-            ⌜ length f0.(f_locs) >= 4 ⌝ ∗
-            ⌜ (0 <= v)%Z ⌝ ∗                                   
-            ⌜ (v + 4 + length s * 4 ≤ Wasm_int.Int32.max_unsigned)%Z ⌝ ∗
-            isStack v s n ∗
-            stackAll s Φ ∗
-            ⌜ f0.(f_inst).(inst_types) !! 1 = Some (Tf [T_i32] [T_i32]) ⌝ ∗
-
-            ⌜ f0.(f_inst).(inst_tab) !! 0 = Some j0 ⌝ ∗
-            (N.of_nat j0) ↦[wt][ N.of_nat (Wasm_int.nat_of_uint i32m f) ] (Some a) ∗
-            na_inv logrel_nais γ ((N.of_nat a) ↦[wf] cl) ∗
-             ⌜ match cl with FC_func_native _ t _ _ => t | FC_func_host t _ => t end 
-          = Tf [T_i32] [T_i32] ⌝ ∗  
-            (∀ (u : i32) (fc : frame),
-                {{{ Φ u ∗
-                      ⌜ f_inst f0 = f_inst fc ⌝ ∗
-                       ↪[frame] fc ∗
-                       na_own logrel_nais ⊤
-                  }}}
-                  [ AI_basic (BI_const (VAL_int32 u)) ;
-                    AI_invoke a ] @ E
-                  {{{ w, (⌜ w = trapV ⌝ ∨ ((∃ v, ⌜ w = immV [VAL_int32 v] ⌝ ∗ Ψ u v)))
-                           ∗ na_own logrel_nais ⊤ ∗ ↪[frame] fc}}}) ∗
-            na_own logrel_nais ⊤ ∗ ↪[frame] f0 }}}
-    to_e_list stack_map @ E
-    {{{ w, (⌜ w = trapV ⌝ ∨ (⌜ w = immV [] ⌝ ∗
-                                        (∃ s', isStack v s' n ∗ stackAll2 s s' Ψ)))
-             ∗ (N.of_nat j0) ↦[wt][ N.of_nat (Wasm_int.nat_of_uint i32m f) ] (Some a)
-             ∗ (∃ f1, ↪[frame] f1 ∗ na_own logrel_nais ⊤ ∗ ⌜ f_inst f0 = f_inst f1 ⌝ )
-    }}}.
-Proof.
-  intros Hsub.
-  iIntros "!>" (Ξ) "(%Hinstmem & %Hlocs0 & %Hlocs1 & %Hlocs & %Hvb & %Hv & Hs & HΦ & %Htypes & %Htab & Htab & #Hcl & %Hcl & #Hspec & Hinv & Hf) HΞ" => /=.
-  rewrite separate4.
-  iApply wp_seq.
-  instantiate (1 := λ x,  (⌜ x = immV [] ⌝ ∗ isStack v s n ∗ ↪[frame] f0)%I).
-  iSplitR; first by iIntros "(%H & _)".
-  iSplitL "Hs Hf"; first by iApply (is_stack_valid with "[$Hs $Hf]").
-  iIntros (w) "(-> & Hs & Hf)".
-  simpl.
-  iApply wp_wand_r.
-  iSplitR "HΞ" ; last first.
-  iIntros (w) "H".
-  iApply "HΞ".
-  iExact "H".
-  iApply wp_wasm_empty_ctx.
-  rewrite (separate1 (AI_basic _)).
-  iApply wp_seq_can_trap_ctx.
-  iSplitR; last first.
-  iFrame "Hf".
-  iSplitR; last first.
-  iSplitR "Hs HΦ".
-  iIntros "Hf".
-  iApply wp_wand_r. iSplitL "Hf". iApply wp_get_local => //.
-  instantiate (1 := λ x, ⌜x = immV [value_of_int v]⌝%I) => //.
-  iIntros (w) "[-> Hf]".
-  iSplitR. iRight. by instantiate (1 := λ x, ⌜ x = immV _ ⌝%I).
-  iExists f0 ; iFrame.
-  iCombine "Htab Hinv" as "H".
-  instantiate (1 := λ x, (⌜ x = f0 ⌝ ∗ _)%I).
-  iSplit ; first done. iExact "H". 
-  iIntros (w f2) "(-> & Hf & [-> HΦf])".
-  iSimpl.
-  rewrite (separate2 (AI_basic _)).
-  iApply wp_seq_can_trap_ctx.
-  iSplitR ; last first. 
-  iFrame "Hf".
-  iSplitR ; last first.
-  iSplitL "Hs HΦf".
-  iIntros "Hf". iApply wp_wand_r. iSplitR "HΦf". iApply wp_load => // ; last first.
-  unfold isStack.
-  iDestruct "Hs" as "(% & % & Hn & ?)".
-  iDestruct (i32_wms with "Hn") as "Hn".
-  rewrite N.add_0_r.
-  simpl.
-  rewrite Wasm_int.Int32.Z_mod_modulus_eq.
-  rewrite Z.mod_small.
-  unfold bits.
-  instantiate (1 := VAL_int32 _) => /=.
-  iFrame.
-  iNext.
-  instantiate ( 1 := λ x, (⌜ x = immV [value_of_int (v + 4 + length s * 4)] ⌝ ∗
-                                     ⌜(two16 | v)%Z⌝ ∗
-                                     ⌜(length s < two14)%Z⌝ ∗
-                                     ([∗ list] i↦w ∈ s, N.of_nat n ↦[i32][ Z.to_N (v + 4 + length s * 4 - 4 - 4 * i)] w) ∗
-      (∃ bs : seq.seq byte, ⌜Z.of_nat (length bs) = (two16 - 4 - length s * 4)%Z⌝ ∗
-                                                                              N.of_nat n↦[wms][Z.to_N (v + 4 + length s * 4)]bs))%I).
-  iFrame.
-  done.
-  unfold Wasm_int.Int32.max_unsigned in Hv ; lia.
-  done.
-  iIntros (w) "[[[-> Hs] Hn] Hf]".
-  iSplitR "Hf HΦf". iRight. instantiate (1 := λ x, (⌜ x = immV _ ⌝ ∗ _ ∗ _)%I).
-  iSplitR ; first done. iSplitL "Hs". iExact "Hs". iExact "Hn".
-  iExists _ ; iFrame. instantiate (1 := λ x, (⌜ x = f0 ⌝ ∗ _ )%I).
-  iSplit ; first done. iExact "HΦf".
-  iIntros (w f1) "((-> & H & Hn) & Hf & [-> HΦf])".
-  iSimpl. rewrite (separate2 (AI_basic _)).
-  iApply wp_seq_can_trap_ctx.
-  iSplitR ; last first.
-  iFrame "Hf". iSplitR ; last first.
-  iSplitL "HΦf".
-  iIntros "Hf".
-  iApply wp_wand_r ; iSplitL "Hf". iApply wp_set_local => //.
-  by instantiate (1 := λ x, ⌜x = immV []⌝%I).
-  iIntros (w) "[-> Hf]".
-  iSplitR. iRight. by instantiate (1 := λ x, ⌜ x = immV [] ⌝%I).
-  iExists _ ; iFrame. instantiate (1 := λ x, (⌜ x = {| f_locs := _ ; f_inst := f_inst f0 |} ⌝∗ _)%I).
-  iSplit ; first done. iExact "HΦf".
-  iIntros (w f1) "(-> & Hf & [-> HΦf])". iSimpl.
-  rewrite (separate1 (AI_basic _)).
-  iApply wp_seq_can_trap_ctx.
-  iSplitR ; last first.
-  iFrame "Hf". iSplitR ; last first.
-  iSplitL "HΦf". 
-  iIntros "Hf". iApply wp_wand_r. iSplitL "Hf".
-  iApply (wp_get_local with "[] [$Hf]") => //=.
-  unfold set_nth.
-  destruct (f_locs f0) ; first by inversion Hlocs0.
-  destruct l ; first by inversion Hlocs1.
-  simpl in Hlocs1.
-  inversion Hlocs1 ; subst.
-  done.
-  by instantiate (1 := λ x, ⌜x = immV [value_of_int v]⌝%I).
-  iIntros (w) "[-> Hf]".
-  iSplitR. iRight. by instantiate (1 := λ x, ⌜ x = immV _ ⌝%I).
-  iExists _ ; iFrame. instantiate (1 := λ x, (⌜ x = {| f_locs := _ ; f_inst := _ |} ⌝ ∗ _)%I).
-  iSplit ; first done. iExact "HΦf".
-  iIntros (w f1) "(-> & Hf & [-> HΦf])". iSimpl.
-  rewrite (separate3 (AI_basic _)).
-  iApply wp_seq_can_trap_ctx.
-  iSplitR ; last first.
-  iFrame "Hf".
-  iSplitR ; last first.
-  iSplitL "HΦf".
-  iIntros "Hf". iApply wp_wand_r ; iSplitL "Hf".
-  iApply (wp_binop with "Hf") => //.
-  by instantiate (1 := λ x, ⌜ x = immV [_] ⌝%I).
-  iIntros (w) "[-> Hf]".
-  iSplitR. iRight.
-  by instantiate (1 := λ x, ⌜ x = immV _ ⌝%I).
-  iExists _ ; iFrame. instantiate (1 := λ x, (⌜ x = {| f_locs := _ ; f_inst := _ |}⌝ ∗ _)%I).
-  iSplit ; first done. iExact "HΦf". iIntros (w f1) "(-> & Hf & [-> HΦf])". iSimpl.
-  rewrite (separate2 (AI_basic _)).
-  iApply wp_seq_can_trap_ctx. 
-  iSplitR ; last first.
-  iFrame "Hf".
-  iSplitR ; last first.
-  iSplitL "HΦf".
-  iIntros "Hf". iApply wp_wand_r ; iSplitL "Hf".
-  iApply wp_set_local => //=.
-  simpl.
-  rewrite length_is_size size_set_nth.
-  rewrite length_is_size in Hlocs.
-  unfold ssrnat.maxn.
-  destruct (ssrnat.leq _ _) ; lia.
-  by instantiate (1 := λ x, ⌜x = immV []⌝%I).
-  iIntros (w) "[-> Hf]".
-  iSplitR. iRight. by instantiate (1 := λ x, ⌜ x = immV [] ⌝%I).
-  iExists _ ; iFrame. instantiate (1 := λ x, (⌜ x = {| f_locs := _ ; f_inst := _ |} ⌝∗ _)%I).
-  iSplit ; first done. iExact "HΦf".
-  iIntros (w f1) "(-> & Hf & [-> HΦf])". simpl.
-  rewrite - (app_nil_l [AI_basic (BI_block _ _)]).
-  iApply (wp_block_ctx with "Hf") => //.
-  iIntros "!> Hf".
-  iSimpl.
-  rewrite - (cat0s [AI_basic (BI_loop _ _)]) - (cats0 [AI_basic (BI_loop _ _)]).
-  iApply wp_label_push ; first done.
-  rewrite - (app_nil_l [AI_basic (BI_loop _ _)]).
-  iApply (wp_loop_ctx with "Hf") => //.
-  iIntros "!> Hf".
-  simpl.
-  rewrite - (cat0s (AI_basic (BI_get_local 2) :: _)).
-  rewrite - (cats0 [AI_basic _;_;_;_;_;_;_;_;_;_;_;_;_;_;_]). 
-  iApply wp_label_push ; first done.
-  unfold Wasm_int.Int32.iadd, Wasm_int.Int32.add.
-  rewrite Wasm_int.Int32.unsigned_repr ; last lia.
-  rewrite Wasm_int.Int32.unsigned_repr ; last by unfold Wasm_int.Int32.max_unsigned,
-      Wasm_int.Int32.modulus, Wasm_int.Int32.wordsize, Integers.Wordsize_32.wordsize.
-  iAssert (∀ (j :nat) s', ⌜ j <= length s ⌝ -∗ ⌜ length s' = length s - j ⌝ -∗ ↪[frame] {|
-                    f_locs :=
-                      set_nth (VAL_int32 (Wasm_int.Int32.repr (v + 4 )))
-                        (set_nth
-                           (VAL_int32 (Wasm_int.Int32.repr (v + 4 + length s * 4)))
-                           (f_locs f0) 3
-                           (VAL_int32 (Wasm_int.Int32.repr (v + 4 + length s * 4)))) 2
-                        (VAL_int32 (Wasm_int.Int32.repr (v + 4 + (length s - j%Z) * 4)));
-                    f_inst := f_inst f0
-                    |} -∗
-                    isStack v (take j s ++ s') n -∗ 
-                    stackAll (take j s) Φ -∗
-                    stackAll2 (drop j s) s' Ψ -∗
-                    na_own logrel_nais ⊤ -∗
-                    N.of_nat j0 ↦[wt][N.of_nat (Z.to_nat (Wasm_int.Int32.unsigned f))]Some a -∗
-                    WP [AI_basic (BI_get_local 2); AI_basic (BI_get_local 3);
-     AI_basic (BI_relop T_i32 (Relop_i (ROI_ge SX_U))); AI_basic (BI_br_if 1);
-     AI_basic (BI_get_local 2); AI_basic (BI_get_local 2); AI_basic (BI_get_local 2);
-     AI_basic (BI_load T_i32 None N.zero N.zero); AI_basic (BI_get_local 0);
-     AI_basic (BI_call_indirect 1); AI_basic (BI_store T_i32 None N.zero N.zero);
-     AI_basic (i32const 4); AI_basic (BI_binop T_i32 (Binop_i BOI_add));
-     AI_basic (BI_set_local 2); AI_basic (BI_br 0)] @  E
-  CTX
-  2;
-  push_base (LH_rec [] 0 [] (LH_base [] []) []) 0
-    [AI_basic
-       (BI_loop (Tf [] [])
-          [BI_get_local 2; BI_get_local 3; BI_relop T_i32 (Relop_i (ROI_ge SX_U));
-          BI_br_if 1; BI_get_local 2; BI_get_local 2; BI_get_local 2;
-          BI_load T_i32 None N.zero N.zero; BI_get_local 0; 
-          BI_call_indirect 1; BI_store T_i32 None N.zero N.zero; 
-          i32const 4; BI_binop T_i32 (Binop_i BOI_add); BI_set_local 2; 
-          BI_br 0])] [] []
-    {{ v0, (⌜v0 = trapV⌝ ∨ ⌜v0 = immV []⌝ ∗
-      (∃ s' : seq.seq Wasm_int.Int32.T, isStack v s' n ∗ stackAll2 s s' Ψ)) ∗
-     N.of_nat j0↦[wt][N.of_nat (Z.to_nat (Wasm_int.Int32.unsigned f))]
-     Some a ∗
-     (∃ f1 : frame,  ↪[frame]f1 ∗ na_own logrel_nais ⊤ ∗ ⌜f_inst f0 = f_inst f1⌝)  }})%I as "Hloop".
-  { iIntros (j).
-    iInduction j as [|j] "IHj".
-    { iIntros (s') "%Hj %Hs' Hf Hs HΦ HΨ Hown Htab".
-      rewrite (separate1 (AI_basic (BI_get_local 2))).
-      iApply wp_seq_can_trap_ctx. 
-      iSplitR ; last first.
-      iFrame "Hf".
-      iSplitR ; last first.
-      iSplitL "Htab Hcl Hown".
-      iIntros "Hf".
-      iApply wp_wand_r ; iSplitL "Hf".
-      iApply (wp_get_local with "[] [$Hf]").
-      simpl. by rewrite set_nth_read.
-      by instantiate ( 1 := λ x, ⌜x = immV _⌝%I).
-      iIntros (w) "[-> Hf]".
-      iSplitR. iRight.
-      by instantiate (1 := λ x, ⌜ x = immV _ ⌝%I).
-      iExists _ ; iFrame. instantiate (1 := λ x, (⌜ x = {| f_locs := _ ; f_inst := _ |} ⌝ ∗ _)%I).
-      iSplit ; first done. iCombine "Htab Hown" as "H". iExact "H".
-      iIntros (w f1) "(-> & Hf & [-> HΦf])". iSimpl.
-      rewrite (separate2 _ (AI_basic (BI_get_local 3))).
-      iApply wp_seq_can_trap_ctx.
-      iSplitR ; last first.
-      iFrame "Hf".
-      iSplitR ; last first.
-      iSplitL "HΦf".
-      iIntros "Hf". rewrite (separate1 _ [AI_basic (BI_get_local 3)]).
-      iApply wp_val_can_trap => //.
-      iSplitR ; last first.
-      iFrame "Hf". iIntros "Hf".
-      iApply wp_wand_r.
-      iSplitL "Hf".
-      iApply (wp_get_local with "[] [$Hf]").
-      simpl.
-      destruct (f_locs f0) ; first by inversion Hlocs.
-      destruct l ; first by inversion Hlocs1.
-      destruct l ; first by simpl in Hlocs ; lia.
-      simpl.
-      by rewrite set_nth_read.
-      by instantiate (1 := λ x, ⌜x = immV _⌝%I).
-      iIntros (w) "[-> Hf]".
-      iSplitR. iRight.
-      by instantiate (1 := λ x, ⌜ x = immV _⌝%I).
-      iExists _ ; iFrame. instantiate (1 := λ x, (⌜ x = {| f_locs := _ ; f_inst := _ |} ⌝ ∗ _)%I).
-      iSplit ; first done. iExact "HΦf".
-      by iIntros "%".
-      iIntros (w f1) "(-> & Hf & [-> HΦf])". rewrite Z.sub_0_r.
-      iSimpl.
-      rewrite (separate3 _ _ (AI_basic (BI_relop _ _))).
-      iApply wp_seq_can_trap_ctx.
-      iSplitR ; last first.
-      iFrame "Hf". iSplitR ; last first.
-      iSplitL "HΦf".
-      iIntros "Hf".
-      iApply wp_wand_r ; iSplitL "Hf".
-      iApply (wp_relop with "Hf").
-      simpl.
-      unfold Wasm_int.Int32.ltu.
-      rewrite Wasm_int.Int32.unsigned_repr.
-      rewrite Coqlib.zlt_false.
-      simpl.
-      done.
-      lia.
-      split ; try lia.
-      exact Hv.
-      by instantiate (1 := λ x, ⌜ x = immV _ ⌝%I).
-      iIntros (w) "[-> Hf]".
-      iSplitR. iRight. by instantiate (1 := λ x, ⌜ x = immV _ ⌝%I).
-      iExists _ ; iFrame. instantiate (1 := λ x, (⌜ x = {| f_locs := _ ; f_inst := _ |} ⌝ ∗ _)%I).
-      iSplit ; first done. iExact "HΦf".
-      iIntros (w f1) "(-> & Hf & (-> & Htab & Hown))". iSimpl.
-      rewrite - (app_nil_l (AI_basic (i32const 1) :: _)).
-      rewrite (separate2 _ (AI_basic (BI_br_if 1))).
-      iApply wp_base_push ; first done.
-      iApply (wp_br_if_true_ctx with "Hf").
-      done.
-      iIntros "!> Hf".
-      rewrite - (app_nil_l [AI_basic (BI_br 1)]).
-      iApply (wp_br_ctx with "Hf") => //.
-      iIntros "!> Hf".
-      iApply wp_value.
-      unfold IntoVal.
-      by apply of_to_val.
-      (*      iApply "HΞ". *)
-      iFrame. iSplitR "Hf". iRight. iSplit ; first done.
-      iExists s'.
-      unfold take.
-      unfold drop.
-      iFrame.
-      iExists _.
-      iFrame.
-      done.
-      all : try by iIntros (f1) "(Hf & -> & Htab & Hown)" ; 
-      iFrame ; iSplitR ; [by iLeft | by iExists _ ; iFrame]. 
-      all : try by iIntros "%".
-    }
-  iIntros (s') "%Hj %Hs' Hf Hs HΦ HΨ Hown Htab".
-  destruct s as [|v0 s]; first by inversion Hj.
-  cut (exists ys y, v0 :: take j s = ys ++ [y]) ;
-  [ intro Htail ; destruct Htail as (ys & y & Htail) |
-    exists (removelast (v0 :: take j s)) ;
-    exists (List.last (v0 :: take j s) (Wasm_int.Int32.repr 1)) ;
-    apply app_removelast_last ;
-    apply not_eq_sym ; apply nil_cons ].
-  simpl in Hv.
-  simpl in Hj.
-  assert (j `min` length s = j) as Hjmin.
-  { remember (length s) as x. rewrite - Heqx in Hj.
-    lia. } 
-  rewrite (separate1 (AI_basic (BI_get_local 2))).
-  iApply wp_seq_can_trap_ctx.
-  iSplitR ; last first.
-  iFrame "Hf". iSplitR ; last first.
-  iSplitL "Hcl Htab Hown".
-  iIntros "Hf". 
-  iApply wp_wand_r. iSplitL "Hf". iApply (wp_get_local with "[] [$Hf]").
-  simpl. by rewrite set_nth_read.
-  by instantiate ( 1 := λ x, ⌜x = immV _⌝%I).
-  iIntros (w) "[-> Hf]".
-  iSplitR. iRight. by instantiate (1 := λ x, ⌜ x = immV _ ⌝%I).
-  iExists _ ; iFrame. instantiate (1 := λ x, (⌜ x = {| f_locs := _ ; f_inst := _ |} ⌝ ∗ _)%I).
-  iSplit ; first done. iCombine "Htab Hown" as "H". iExact "H".
-  iIntros (w f1) "(-> & Hf & -> & HΦf)". iSimpl.
-  rewrite (separate2 _ (AI_basic (BI_get_local 3))).
-  iApply wp_seq_can_trap_ctx.
-  iSplitR ; last first.
-  iFrame "Hf". iSplitR ; last first.
-  iSplitL "HΦf".
-  rewrite (separate1 _ [AI_basic (BI_get_local 3)]).
-  iIntros "Hf". iApply wp_val_can_trap => //.
-  iSplitR ; last first.
-  iFrame "Hf". iIntros "Hf".
-  iApply wp_wand_r.
-  iSplitL "Hf".
-  iApply (wp_get_local with "[] [$Hf]").
-  simpl.
-  destruct (f_locs f0) ; first by inversion Hlocs.
-  destruct l ; first by inversion Hlocs1.
-  destruct l ; first by simpl in Hlocs ; lia.
-  simpl.
-  by rewrite set_nth_read.
-  by instantiate (1 := λ x, ⌜x = immV _⌝%I).
-  iIntros (w) "[-> Hf]".
-  iSplitR. iRight. by instantiate ( 1 := λ x, ⌜ x = immV _ ⌝%I).
-  iExists _ ; iFrame. instantiate (1 := λ x, (⌜ x = {| f_locs := _ ; f_inst := _ |} ⌝ ∗ _ )%I).
-  iSplit ; first done. iExact "HΦf".
-  by iIntros "%".
-  iIntros (w f1) "(-> & Hf & -> & HΦf)". iSimpl.
-  rewrite (separate3 _ _ (AI_basic (BI_relop _ _))).
-  iApply wp_seq_can_trap_ctx.
-  iSplitR ; last first.
-  iFrame "Hf". iSplitR ; last first.
-  iSplitL "HΦf".
-  iIntros "Hf". iApply wp_wand_r. iSplitL "Hf".
-  iApply (wp_relop with "Hf").
-  simpl.
-  unfold Wasm_int.Int32.ltu.
-  rewrite Wasm_int.Int32.unsigned_repr.
-  rewrite Wasm_int.Int32.unsigned_repr.
-  rewrite Coqlib.zlt_true.
-  simpl.
-  done.
-  lia.
-  lia.
-  lia.
-  by instantiate (1 := λ x, ⌜ x = immV _ ⌝%I).
-  iIntros (w) "[-> Hf]".
-  iSplitR. iRight. by instantiate (1 := λ x, ⌜ x = immV _ ⌝%I).
-  iExists _ ; iFrame. instantiate (1 := λ x, (⌜ x = {| f_locs := _ ; f_inst := _ |} ⌝ ∗ _)%I).
-  iSplit ; first done. iExact "HΦf".
-  iIntros (w f1) "(-> & Hf & -> & HΦf)". iSimpl.
-  rewrite (separate2 (AI_basic (BI_const (VAL_int32 _)))).
-  iApply wp_seq_can_trap_ctx.
-  iSplitR ; last first.
-  iFrame "Hf". iSplitR ; last first.
-  iSplitL "HΦf".
-  iIntros "Hf". iApply wp_wand_r ; iSplitL "Hf".
-  iApply (wp_br_if_false with "Hf").
-  done.
-  iNext.
-  by instantiate (1 := λ x, ⌜ x = immV [] ⌝%I).
-  iIntros (w) "[-> Hf]".
-  iSplitR. iRight. by instantiate (1 := λ x, ⌜ x = immV [] ⌝%I).
-  iExists _ ; iFrame. instantiate (1 := λ x, (⌜ x = {| f_locs := _ ; f_inst := _ |} ⌝ ∗ _ )%I).
-  iSplit ; first done. iExact "HΦf".
-  iIntros (w f1) "(-> & Hf & -> & HΦf)". iSimpl.
-  rewrite (separate1 (AI_basic (BI_get_local 2)) [_;_;_;_;_;_;_;_;_;_]).
-  iApply wp_seq_can_trap_ctx.
-  iSplitR ; last first.
-  iFrame "Hf". iSplitR ; last first.
-  iSplitL "HΦf".
-  iIntros "Hf". 
-  iApply wp_wand_r ; iSplitL "Hf".
-  iApply (wp_get_local with "[] [$Hf]") => /=.
-  by rewrite set_nth_read.
-  by instantiate (1 := λ x, ⌜x = immV _⌝%I).
-  iIntros (w) "[-> Hf]".
-  iSplitR. iRight. by instantiate (1 := λ x, ⌜ x = immV _ ⌝%I).
-  iExists _ ; iFrame. instantiate (1 := λ x, (⌜ x = {| f_inst := _ ; f_locs := _ |} ⌝ ∗ _)%I).
-  iSplit ; first done. iExact "HΦf".
-  iIntros (w f1) "(-> & Hf & -> & HΦf)". iSimpl.
-  rewrite (separate2 (AI_basic (i32const (v + 4 + _ * 4)))).
-  iApply wp_seq_can_trap_ctx.
-  iSplitR ; last first.
-  iFrame "Hf". iSplitR ; last first.
-  iSplitL "HΦf".
-  iIntros "Hf".
-  rewrite (separate1 (AI_basic (i32const (v + 4 + _ * 4)))).
-  iApply wp_val_can_trap. 
-  iSplitR ; last first.
-  iFrame "Hf". iIntros "Hf". iApply wp_wand_r.
-  iSplitL "Hf".
-  iApply (wp_get_local with "[] [$Hf]") => /=.
-  by rewrite set_nth_read.
-  by instantiate (1 := λ x, ⌜x = immV _⌝%I).
-  iIntros (w) "[-> Hf]".
-  iSplitR. iRight. by instantiate (1 := λ x, ⌜ x = immV _ ⌝%I).
-  iExists _ ; iFrame. instantiate (1 := λ x, (⌜ x = {| f_locs := _ ; f_inst := _ |} ⌝ ∗ _)%I).
-  iSplit ; first done. iExact "HΦf".
-  by iIntros "%".
-  iIntros (w f1) "(-> & Hf & -> & HΦf)". iSimpl.
-  rewrite (separate3 (AI_basic (i32const (v + 4 + _ * 4)))).
-  iApply wp_seq_can_trap_ctx.
-  iSplitR ; last first.
-  iFrame "Hf". iSplitR ; last first.
-  iSplitL "HΦf". iIntros "Hf".
-  rewrite (separate2 (AI_basic (i32const (v + 4 + _ * 4)))).
-  iApply wp_val_can_trap.
-  iSplitR ; last first.
-  iFrame "Hf". iIntros "Hf".
-  iApply wp_wand_r.
-  iSplitL.
-  iApply wp_val_can_trap.
-  iSplitR ; last first.
-  iFrame "Hf". iIntros "Hf".
-  iApply wp_wand_r.
-  iSplitL "Hf". iApply (wp_get_local with "[] [$Hf]") => /=.
-  by rewrite set_nth_read.
-  by instantiate (1 := λ x, ⌜x = immV _⌝%I).
-  iIntros (w) "[-> Hf]".
-  iSplitR. iRight. by instantiate (1 := λ x, ⌜ x = immV _ ⌝%I).
-  iExists _ ; iFrame. instantiate (1 := λ x, (⌜ x = {| f_inst := _ ; f_locs := _ |} ⌝ ∗ _)%I).
-  iSplit ; first done. iExact "HΦf".
-  by iIntros "%".
-  iIntros (w) "[[-> | ->] Hf]".
-  iSplitR. by iLeft. iExact "Hf".
-  iSplitR. iRight. by instantiate (1 := λ x, ⌜ x = immV _ ⌝%I).
-  iExact "Hf".
-  by iIntros "%".
-  iIntros (w f1) "(-> & Hf & -> & HΦf)". iSimpl.
-  rewrite (separate4 (AI_basic (i32const (v + 4 + _ * 4)))).
-  iApply wp_seq_can_trap_ctx.
-  iSplitR ; last first.
-  iFrame "Hf". iSplitR ; last first.
-  iSplitL "HΦf Hs".
-  iIntros "Hf".
-  iApply wp_val_can_trap.
-  iSplitR ; last first.
-  iFrame "Hf". iIntros "Hf". 
-  iApply wp_wand_r ; iSplitL. iApply wp_val_can_trap.
-  iSplitR ; last first.
-  iFrame "Hf". iIntros "Hf". iApply wp_wand_r.
-  iSplitR "HΦf".
-  iApply wp_load ; last first.
-  iFrame.
-  unfold isStack.
-  iDestruct "Hs" as "(Hdiv & Hlen & Hn & Hl & Hbs)".
-  rewrite cat_app.
-  iDestruct (big_sepL_app with "Hl") as "[Hs Hs']".
-  rewrite app_length.
-  rewrite Hs'.
-  rewrite take_length.
-  replace (S j `min` length (v0 :: s)) with (S j) ; last by simpl ; lia.
-  unfold take ; fold (take (A := value)).
-  rewrite Htail.
-  iDestruct (big_sepL_app with "Hs") as "[Hs H]".
-  iDestruct "H" as "[H _]".
-  iDestruct (i32_wms with "H") as "H" => //.
-  rewrite Nat.add_0_r.
-  rewrite N.add_0_r.
-  replace (Wasm_int.N_of_uint i32m (Wasm_int.Int32.repr (v + 4 + (S (length s) - S j) * 4)))
-    with (Z.to_N (v + 4 + (S (length s) - S j) * 4)).
-  replace (S j + (length (v0 :: s) - S j)) with (length (v0 :: s)) ; last by simpl ; lia.
-  replace (v + 4 + length (v0 :: s) * 4 - 4 - 4 * length ys)%Z
-    with (v + 4 + length (v0 :: s) * 4 - S (length ys) * 4)%Z ; last lia.
-  replace (S (length ys)) with (length (ys ++ [y])) ;
-    last by rewrite app_length ; simpl ; lia.
-  rewrite (cat_app ys [y]).
-  rewrite - Htail.
-  simpl.
-  rewrite firstn_length.
-  rewrite Hjmin.
-  rewrite (Z.mul_sub_distr_r (S (length s)) (S j) 4).
-  simpl in Hj.
-  remember (length s) as x.
-  rewrite - Heqx.
-  replace (v + 4 + S x * 4 - S j * 4)%Z
-    with (v + 4 + (S x * 4 - S j * 4))%Z ;
-    last lia.
-  rewrite Wasm_int.Int32.Z_mod_modulus_eq Z.mod_small.
-  instantiate (1 := VAL_int32 _).
-  iSplitR "H" ; last iExact "H".
-  iNext.
-  subst x.
-  instantiate ( 1 := λ x, (⌜ x = immV [VAL_int32 y] ⌝ ∗ ⌜ (two16 | v)%Z ⌝ ∗ ⌜ (S (length s) < two14)%Z ⌝ ∗ N.of_nat n ↦[i32][ Z.to_N v] Wasm_int.Int32.repr (v + 4 + S (length s) * 4) ∗  (∃ bs : seq.seq byte, ⌜ Z.of_nat (length bs) = (two16 - 4 - S (length s) * 4)%Z⌝ ∗
-            N.of_nat n↦[wms][Z.to_N (v + 4 + S (length s) * 4)]bs) ∗ ([∗ list] k↦y0 ∈ s', N.of_nat n
-                              ↦[i32][ Z.to_N
-                                        (v + 4 + S (length s) * 4 - 4 - 4 * S (j + k))] y0) ∗ [∗ list] k↦y0 ∈ ys, N.of_nat n
-                             ↦[i32][ Z.to_N (v + 4 + S (length s) * 4 - 4 - 4 * k)] y0)%I).
-  iFrame.
-  done.
-  simpl.
-  unfold Wasm_int.Int32.max_unsigned in Hv ; rewrite - Heqx in Hv ; lia.
-  simpl.
-  rewrite Wasm_int.Int32.Z_mod_modulus_eq.
-  rewrite Z.mod_small.
-  done.
-  unfold Wasm_int.Int32.max_unsigned in Hv ; lia.
-  done.
-  done.
-  iIntros (w) "[[[-> H1] H2] Hf]".
-  iSplitR "Hf HΦf". 
-  iRight. iSimpl.
-  instantiate (1 := λ x, (⌜ x = immV _ ⌝ ∗
-                                     ( ⌜(two16 | v)%Z⌝ ∗ ⌜(S (length s) < two14)%Z⌝ ∗ N.of_nat n ↦[i32][ Z.to_N v] Wasm_int.Int32.repr (v + 4 + S (length s) * 4) ∗
-         (∃ bs : seq.seq byte, ⌜Z.of_nat (length bs) = (two16 - 4 - S (length s) * 4)%Z⌝ ∗
-            N.of_nat n↦[wms][Z.to_N (v + 4 + S (length s) * 4)]bs) ∗
-         ([∗ list] k↦y0 ∈ s', N.of_nat n
-                              ↦[i32][ Z.to_N
-                                        (v + 4 + S (length s) * 4 - 4 - 4 * S (j + k))] y0) ∗
-         ([∗ list] k↦y0 ∈ ys, N.of_nat n
-                                       ↦[i32][ Z.to_N (v + 4 + S (length s) * 4 - 4 - 4 * k)] y0))
-                                     ∗ N.of_nat n↦[wms][Wasm_int.N_of_uint i32m
-                            (Wasm_int.Int32.repr (v + 4 + (length (v0 :: s) - S j) * 4)) +
-                                                          N.zero]bits (VAL_int32 y)
-                                 )%I).
-  iFrame.
-  done.
-  iExists _ ; iFrame.
-  instantiate (1 := λ x, (⌜ x = {| f_locs := _ ; f_inst := _ |} ⌝ ∗ _)%I).
-  iSplit ; first done. iExact "HΦf".
-  by iIntros "[% _]".
-  iIntros (w) "[[ -> | [-> H]] Hf]".
-  iSplitR. by iLeft. iExact "Hf".
-  iSplitL "H". iRight. instantiate (1 := λ x, (⌜ x = immV _ ⌝ ∗ _)%I).
-  iSplit ; first done. iExact "H".
-  iExact "Hf".
-  by iIntros "[% _]".
-  iIntros (w f1) 
-          "((-> & (Hdiv & Hlen & Hv & Hbs & Hs' & Hs) & H) & Hf & -> & HΦf)".
-  iSimpl.
-  rewrite (separate4 (AI_basic (i32const (v + 4 + _ * 4)))).
-  iApply wp_seq_can_trap_ctx.
-  iSplitR ; last first.
-  iFrame "Hf". iSplitR ; last first.
-  iSplitL "HΦf". iIntros "Hf". 
-  iApply wp_val_can_trap.
-  iSplitR ; last first.
-  iFrame "Hf". iIntros "Hf".
-  iApply wp_wand_r. iSplitL.
-  iApply wp_val_can_trap.
-  iSplitR ; last first.
-  iFrame "Hf". iIntros "Hf".
-  iApply wp_wand_r. iSplitL.
-  iApply wp_val_can_trap.
-  iSplitR ; last first.
-  iFrame "Hf".
-  iIntros "Hf".
-  iApply wp_wand_r.
-  iSplitL "Hf".
-  iApply (wp_get_local with "[] [$Hf]") => /=.
-  destruct (f_locs f0) ; inversion Hlocs0.
-  simpl. done.
-  by instantiate (1 := λ x, ⌜x = immV _⌝%I).
-  iIntros (w) "[-> Hf]".
-  iSplitR. iRight. by instantiate (1 := λ x, ⌜ x = immV _ ⌝%I).
-  iExists _ ; iFrame. instantiate (1 := λ x, (⌜ x = {| f_locs := _ ; f_inst := _ |} ⌝ ∗ _)%I).
-  iSplit ; first done. iExact "HΦf".
-  by iIntros "%".
-  iIntros (w) "[[-> | ->] Hf]".
-  iSplitR. by iLeft. iExact "Hf".
-  iSplitR. iRight. by instantiate (1 := λ x, ⌜ x = immV _ ⌝%I).
-  iExact "Hf".
-  by iIntros "%".
-  iIntros (w) "[[ -> | ->] Hf]".
-  iSplitR. by iLeft. iExact "Hf".
-  iSplitR. iRight. by instantiate (1 := λ x, ⌜ x = immV _ ⌝%I).
-  iExact "Hf".
-  by iIntros "%".
-  iIntros (w f1) "(-> & Hf & -> & Htab & Hown)". iSimpl.
-  rewrite (separate5 (AI_basic (i32const (v + 4 + _ * 4)))).
-  iApply wp_seq_can_trap_ctx.
-  iSplitR ; last first.
-  iFrame "Hf". iSplitR ; last first.
-  iSplitL "HΦ Htab Hown".
-  iIntros "Hf". 
-  iApply wp_val_can_trap.
-  iSplitR ; last first.
-  iFrame "Hf". iIntros "Hf".
-  iApply wp_wand_r. iSplitL.
-  iApply wp_val_can_trap.
-  iSplitR ; last first.
-  iFrame "Hf". iIntros "Hf".
-  iApply wp_wand_r ; iSplitL.
-  unfold take ; fold (take (A := value)).
-  rewrite Htail.
-  iDestruct (stackAll_app with "HΦ") as "(HΦ & Hy & _)".
-  rewrite (separate1 _ [_;AI_basic (BI_call_indirect 1)]).
-  rewrite - (app_nil_r [_ ; AI_basic (BI_call_indirect 1)]).
-  iApply fupd_wp. iMod (na_inv_acc with "Hcl Hown") as "(>Ha & Hown & Hcls)";[auto|solve_ndisj|].
-  iApply wp_wasm_empty_ctx.
-  iApply wp_base_push ; first done.
-  iApply (wp_call_indirect_success_ctx with "Htab Ha Hf").
-  simpl.
-  unfold cl_type.
-  rewrite Hcl.
-  done.
-  simpl.
-  done. iModIntro.
-  iIntros "!> (Htab & Ha & Hf)".
-  iApply wp_base_pull.
-  iApply wp_wasm_empty_ctx.
-  iApply fupd_wp. iMod ("Hcls" with "[$]") as "Hown". simpl.
-  iApply ("Hspec" with "[Hy Hf Hown]").
-  iFrame.
-  iPureIntro => //=.
-  iModIntro. iIntros (w) "H".
-  iCombine "HΦ Htab H" as "H".
-  iExact "H".
-  iIntros (w) "(HΦ & Htab & H & Hown & Hf)".
-  iDestruct "H" as "[-> | H]".
-  iSplitL "HΦ". by iLeft.
-  iExists _ ; iFrame. instantiate (1 := λ x, (⌜ x = {| f_locs := _ ; f_inst := _ |}⌝ ∗ _)%I).
-  iSplit ; first done. iCombine "Htab Hown" as "H".
-  iExact "H".
-  iSplitL "HΦ H". iRight. instantiate (1 := λ x, (∃ v1, ⌜ x = immV _ ⌝ ∗ stackAll ys Φ ∗ Ψ y v1)%I).
-  iDestruct "H" as (v1) "[-> H]".
-  iSimpl.
-  iExists _ ; by iFrame.
-  iExists _ ; iFrame. done.
-  by iIntros "H" ; iDestruct "H" as (v1) "[% _]".
-  iIntros (w) "[[-> | H] Hf]".
-  iSplitR. by iLeft. iExact "Hf".
-  iSplitR "Hf". iRight.
-  iDestruct "H" as (v1) "[-> H]".
-  instantiate (1 := λ x, (∃ v1, ⌜ x = immV _ ⌝ ∗ _)%I).
-  iExists _. iSplit ; first done. iExact "H".
-  iExact "Hf".
-  by iIntros "H" ; iDestruct "H" as (v1) "[% _]".
-  iIntros (w f1) "(H' & Hf & -> & HΦf)". 
-  iDestruct "H'" as (v1) "(-> & HΦ & Hv1)".
-  iSimpl.
-  rewrite (separate4 (AI_basic (i32const (v + 4 + _ * 4)))).
-  iApply wp_seq_can_trap_ctx.
-  iSplitR ; last first.
-  iFrame "Hf". iSplitR ; last first.
-  iSplitL "HΦf H".
-  iIntros "Hf". 
-  iApply wp_val_can_trap.
-  iSplitR ; last first.
-  iFrame "Hf". iIntros "Hf". iApply wp_wand_r.
-  iSplitR "HΦf".
-  iApply wp_store ; last first.
-  simpl.
-  iFrame.
-  iNext.
-  by instantiate (1 := λ x, ⌜ x = immV [] ⌝%I).
-  done.
-  done.
-  done.
-  iIntros (w) "[[-> H] Hf]".
-  iSplitL "H". iRight. 
-  by instantiate (1 := λ x, (⌜ x = immV _ ⌝ ∗ N.of_nat n↦[wms][ _ ] _)%I) ;
-  iFrame.
-  iExists _ ; iFrame. instantiate (1 := λ x, (⌜ x = {| f_locs := _ ; f_inst := _ |} ⌝ ∗ _)%I).
-  iSplit ; first done. iExact "HΦf".
-  by iIntros "[% _]".
-  iIntros (w f1) "([-> H] & Hf & -> & HΦf)".
-  iSimpl.
-  rewrite (separate3 (AI_basic (i32const (v + 4 + _ * 4)))).
-  iApply wp_seq_can_trap_ctx.
-  iSplitR ; last first.
-  iFrame "Hf". iSplitR ; last first.
-  iSplitL "HΦf". iIntros "Hf". 
-  iApply wp_wand_r. iSplitL "Hf". iApply (wp_binop with "Hf").
-  done.
-  by instantiate (1 := λ x, ⌜ x = immV _ ⌝%I).
-  iIntros (w) "[-> Hf]".
-  iSplitR. iRight. by instantiate (1 := λ x, ⌜ x = immV _ ⌝%I).
-  iExists _ ; iFrame. instantiate (1 := λ x, (⌜ x = {| f_locs := _ ; f_inst := _ |} ⌝ ∗ _)%I).
-  iSplit ; first done. iExact "HΦf".
-  iIntros (w f1) "(-> & Hf & -> & HΦf)". iSimpl.
-  rewrite (separate2 (AI_basic (BI_const (VAL_int32 (Wasm_int.Int32.iadd _ _))))).
-  iApply wp_seq_can_trap_ctx.
-  iSplitR ; last first.
-  iFrame "Hf". iSplitR ; last first.
-  iSplitL "HΦf". iIntros "Hf". 
-  iApply wp_wand_r. iSplitL "Hf".
-  iApply (wp_set_local with "[] [$Hf]") => /=.
-  destruct (f_locs f0) ; first done.
-  destruct l ; first done.
-  destruct l ; first by simpl in Hlocs ; lia.
-  destruct l ; first by simpl in Hlocs ; lia.
-  simpl.
-  lia.
-  by instantiate (1 := λ x, ⌜x = immV _⌝%I).
-  iIntros (w) "[-> Hf]".
-  iSplitR. iRight. by instantiate (1 := λ x, ⌜x = immV _⌝%I).
-  iExists _ ; iFrame. instantiate (1 := λ x, (⌜ x = {| f_locs := _ ; f_inst := _ |} ⌝ ∗ _)%I).
-  iSplit ; first done. iExact "HΦf".
-  iIntros (w f1) "(-> & Hf & -> & Htab & Hown)". simpl.
-  rewrite set_nth_write.
-  all : try by iIntros (f1) "(Hf & -> & Htab & Hown)" ; 
-    iFrame ; iSplitR ; [by iLeft | by iExists _ ; iFrame]. 
-  all : try by iIntros "%".
-  all : try by iIntros "[% _]".
-  all : try by iIntros "H" ; iDestruct "H" as (v1) "[% _]".
-  rewrite - (app_nil_l [AI_basic (BI_br 0)]).
-  iApply (wp_br_ctx_nested with "Hf").
-  lia.
-  done.
-  instantiate (1 := LH_rec [] 0 [] (LH_base [] []) []) => //=.
-  done.
-  done.
-  iIntros "!> Hf".
-  iSimpl.
-  rewrite - (app_nil_l [AI_basic (BI_loop _ _)]).
-  iApply (wp_loop_ctx with "Hf") => //.
-  iIntros "!> Hf".
-  simpl.
-  rewrite - (cat0s (AI_basic (BI_get_local 2) :: _)).
-  rewrite - (cats0 [AI_basic _;_;_;_;_;_;_;_;_;_;_;_;_;_;_]). 
-  iApply wp_label_push ; first done.
-  iApply ("IHj" with "[] [] [Hf] [Hv Hbs Hs' Hs H Hlen Hdiv] [HΦ] [HΨ Hv1] Hown Htab").
-  iPureIntro.
-  lia.
-  instantiate (1 := v1 :: s').
-  iPureIntro.
-  simpl.
-  rewrite Hs' => //=.
-  lia.
-  unfold Wasm_int.Int32.iadd, Wasm_int.Int32.add.
-  rewrite Wasm_int.Int32.unsigned_repr.
-  rewrite Wasm_int.Int32.unsigned_repr.
-  remember (length s) as x. rewrite - Heqx.
-  replace (v + 4 + (S x - S j) * 4 + 4)%Z
-    with (v + 4 + (S x - j) * 4)%Z.
-  iExact "Hf".
-  lia.
-  lia.
-  lia.
-  unfold isStack.
-  iFrame.
-  iDestruct "Hlen" as "%".
-  iSplit ; first iPureIntro.
-  rewrite app_length.
-  rewrite firstn_length.
-  replace (j `min` length (v0 :: s)) with j ; last by simpl ; lia.
-  simpl.
-  rewrite Hs'.
-  simpl.
-  lia.
-  iSplitL "Hv".
-  rewrite app_length.
-  rewrite firstn_length.
-  simpl.
-  remember (length s) as x. rewrite - Heqx.
-  replace (j `min` S x) with j ; last by simpl ; lia.
-  simpl.
-  rewrite Hs'.
-  simpl.
-  rewrite - Heqx.
-  replace (j + S (x - j)) with (S (x)) ; last lia.
-  iExact "Hv".
-  iSplitR "Hbs".
-  iApply big_sepL_app.
-  iSplitL "Hs".
-  replace j with (j `min` S j) ; last lia.
-  rewrite - take_take.
-  simpl.
-  rewrite Htail.
-  replace j with (length ys).
-  rewrite take_app.
-  iApply (big_sepL_impl with "Hs").
-  iIntros "!>" (k x) "% H".
-  remember (length s) as z ; rewrite - Heqz.
-  replace (S z) with (length (ys ++ v1 :: s')) ; first done.
-  rewrite app_length.
-  simpl.
-  rewrite Hs'.
-  simpl.
-  rewrite - Heqz.
-  remember (length ys) as zz ; rewrite - Heqzz.
-  replace zz with j ; first lia.
-  specialize (f_equal length Htail) as Hl.
-  simpl in Hl.
-  rewrite app_length in Hl ; simpl in Hl.
-  rewrite firstn_length in Hl.
-  subst z. rewrite Hjmin in Hl. rewrite - Heqzz in Hl. lia.
-  specialize (f_equal length Htail) as Hl.
-  simpl in Hl.
-  rewrite app_length in Hl ; simpl in Hl.
-  rewrite firstn_length in Hl.
-  rewrite Hjmin in Hl.
-  remember (length ys) as zz.
-  rewrite - Heqzz in Hl.
-  lia.
-  iSplitL "H".
-  iApply i32_wms.
-  rewrite Wasm_int.Int32.Z_mod_modulus_eq.
-  rewrite Z.mod_small.
-  rewrite N.add_0_r.
-  rewrite Nat.add_0_r.
-  rewrite app_length.
-  rewrite firstn_length.
-  simpl.
-  remember (length s) as x ; rewrite - Heqx.
-  replace (j `min` S x) with j ; last by simpl ; lia.
-  rewrite Hs'.
-  simpl.
-  rewrite - Heqx.
-  replace (j + S (x - j)) with (S (x)) ; last lia.
-  replace (v + 4 + S x *4 - 4 -4 * j)%Z
-    with  (v + 4 + ( S x - S j) * 4)%Z ; last lia.
-  iExact "H".
-  unfold Wasm_int.Int32.max_unsigned in Hv.
-  lia.
-  iApply (big_sepL_impl with "Hs'").
-  iIntros "!>" (k x) "% H".
-  rewrite app_length.
-  rewrite firstn_length.
-  simpl.
-  remember (length s) as z ; rewrite - Heqz.
-  replace (j `min` S z) with j ; last by simpl ; lia.  
-  rewrite Hs'.
-  simpl.
-  rewrite - Heqz.
-  replace (j + S (z - j)) with (S z) ; last lia.
-  replace (S ( j + k)) with (j + S k) ; last lia.
-  iExact "H".
-  iDestruct "Hbs" as (bs) "[% H]".
-  iExists bs.
-  iSplit ; first iPureIntro.
-  rewrite app_length.
-  rewrite firstn_length.
-  simpl.
-  remember (length s) as x ; rewrite - Heqx.
-  replace (j `min` S x) with j ; last by simpl ; lia.
-  simpl.
-  rewrite Hs'.
-  simpl.
-  lia.
-  rewrite app_length.
-  rewrite firstn_length.
-  simpl.
-  remember (length s) as x ; rewrite - Heqx.
-  replace (j `min` S x) with j ; last by simpl ; lia.
-  simpl.
-  rewrite Hs'.
-  simpl.
-  rewrite - Heqx.
-  replace (j + S (x - j)) with (S x) ; last lia.
-  iExact "H".
-  replace j with (j `min` S j) ; last lia.
-  rewrite - take_take.
-  simpl.
-  rewrite Htail.
-  replace j with (length ys).
-  rewrite take_app.
-  done.
-  specialize (f_equal length Htail) as Hl.
-  simpl in Hl.
-  rewrite app_length in Hl ; simpl in Hl.
-  rewrite firstn_length in Hl.
-  rewrite Hjmin in Hl.
-  remember (length ys) as zz ; rewrite - Heqzz in Hl ;
-    lia.
-  rewrite - (take_drop j s).
-  rewrite app_comm_cons.
-  rewrite Htail.
-  rewrite take_drop.
-  rewrite drop_app_le.
-  replace j with (length ys).
-  rewrite drop_app.
-  simpl.
-  iFrame.
-  specialize (f_equal length Htail) as Hl.
-  simpl in Hl.
-  rewrite app_length in Hl ; simpl in Hl.
-  rewrite firstn_length in Hl.
-  rewrite Hjmin in Hl.
-  remember (length ys) as zz ; rewrite - Heqzz in Hl ;
-    lia.
-  specialize (f_equal length Htail) as Hl.
-  simpl in Hl.
-  rewrite app_length in Hl ; simpl in Hl.
-  rewrite firstn_length in Hl.
-  rewrite app_length.
-  rewrite - Hl.
-  lia. }
-  iDestruct "HΦf" as "(Htab & Hown)".
-  iApply ("Hloop" with "[] [] [Hf] [Hn H] [HΦ] [] Hown Htab").
-  instantiate (1 := length s).
-  iPureIntro ; lia.
-  instantiate (1 := []).
-  iPureIntro ; simpl ; lia.
-  rewrite Z.sub_diag.
-  rewrite Z.mul_0_l.
-  rewrite Z.add_0_r.
-  done.
-  iDestruct "H" as "(% & % & Hs & Hbs)".
-  iSplit ; first done.
-  iSplit ; first iPureIntro.
-  rewrite cats0 firstn_length.
-  rewrite Nat.min_id.
-  exact H0.
-  iSplitL "Hn".
-  iApply i32_wms.
-  rewrite N.add_0_r.
-  rewrite Wasm_int.Int32.Z_mod_modulus_eq.
-  rewrite Z.mod_small.
-  rewrite cats0 firstn_length.
-  rewrite Nat.min_id.
-  done.
-  unfold Wasm_int.Int32.max_unsigned in Hv ; lia.
-  iSplitL "Hs".
-  rewrite cats0 firstn_length.
-  rewrite firstn_all.
-  rewrite Nat.min_id.
-  done.
-  rewrite cats0 firstn_length.
-  rewrite Nat.min_id.
-  done.
-  rewrite firstn_all.
-  done.
-  rewrite drop_all.
-  done.
-  all : try by iIntros (f1) "(Hf & -> & Htab & Hown)" ; 
-    iFrame ; iSplitR ; [by iLeft | by iExists _ ; iFrame]. 
-  all : try by iIntros "%".
-  by iIntros "[% _]".
-Qed. 
 
 End specs.
 
